Move Check: split the files into MoveCheckingDomain (define semantics interfaces and invariant) and MoveCheckingFootprint (defined abstract memory)

rustfrontend/Rusttyping.v
@@ -5,7 +5,8 @@ Require Import Floats.
 Require Import Values.
 Require Import Memory.
 Require Import Ctypes Cop Ctyping.
-Require Import Rusttypes RustOp Rustlight.
+Require Import Rusttypes RustOp Rustlight Rustlightown.
+Require Import RustIR RustIRown.
 Require Import Errors Maps.
 Require Archi.
 
@@ -134,3 +135,202 @@ Definition type_binop (op: binary_operation) (ty1 ty2: type) : res type :=
   | Oge => comparison_type ty1 ty2 "operator >="
   end.
 
+(** * Syntactic type checking  *)
+
+Definition type_deref (ty: type) : res type :=
+  match ty with
+  (* Only support box type to be dereferenced for now *)
+  | Tbox tyelt => OK tyelt
+  (* | Treference _ _ tyelt => OK tyelt *)
+  | _ => Error (msg "type_deref error")
+  end.
+
+Lemma type_deref_some: forall ty1 ty2,
+    type_deref ty1 = OK ty2 ->
+    ty1 = Tbox ty2.
+Proof.
+  destruct ty1; intros; simpl in *; try congruence.
+Qed.
+
+
+(* Some simple type checking (move to Rusttyping.v) *)
+
+(* We do not support array type and reference type for now *)
+Definition valid_type (ty: type) : bool :=
+  match ty with
+  | Tarray _ _
+  | Treference _ _ _
+  | Tfunction _ _ _ _ _ => false
+  | _ => true
+  end.
+
+Definition typenv := PTree.t type.
+
+Section TYPING.
+
+Variable te: typenv.
+Variable ce: composite_env.
+
+Inductive wt_place : place -> Prop :=
+| wt_local: forall id ty
+    (WT1: te ! id = Some ty)
+    (VTY: valid_type ty = true),
+    wt_place (Plocal id ty)
+| wt_deref: forall p ty
+    (WT1: wt_place p)
+    (WT2: type_deref (typeof_place p) = OK ty),
+    (* (VTY: valid_type ty = true), *)
+    wt_place (Pderef p ty)
+| wt_field: forall p ty fid co orgs id
+    (WT1: wt_place p)
+    (WT2: typeof_place p = Tstruct orgs id)
+    (WT3: ce ! id = Some co)
+    (WT4: field_type fid co.(co_members) = OK ty)
+    (WT5: co.(co_sv) = Struct),
+    wt_place (Pfield p fid ty)
+| wt_downcast: forall p ty fid co orgs id
+    (WT1: wt_place p)
+    (WT2: typeof_place p = Tvariant orgs id)
+    (WT3: ce ! id = Some co)
+    (WT4: field_type fid co.(co_members) = OK ty)
+    (WT5: co.(co_sv) = TaggedUnion),
+    wt_place (Pdowncast p fid ty).
+
+Inductive wt_pexpr: pexpr -> Prop :=
+| wt_Eunit:
+  wt_pexpr Eunit
+| wt_Econst_int: forall n sz si,
+    wt_pexpr (Econst_int n (Tint sz si))
+| wt_Econst_float: forall f sz,
+    wt_pexpr (Econst_float f (Tfloat sz))
+| wt_Econst_single: forall f sz,
+    wt_pexpr (Econst_single f (Tfloat sz))
+| wt_Econst_long: forall n si,
+    wt_pexpr (Econst_long n (Tlong si))
+| wt_Eplace: forall p
+    (WTP1: wt_place p),
+    wt_pexpr (Eplace p (typeof_place p))
+| wt_Ecktag: forall p fid orgs id
+    (WTP1: typeof_place p = Tvariant orgs id),
+    wt_pexpr (Ecktag p fid)
+| wt_Eref: forall p org mut
+    (WTP1: wt_place p),
+    wt_pexpr (Eref org mut p (Treference org mut (typeof_place p)))
+| wt_Eunop: forall uop pe ty
+    (WTP1: wt_pexpr pe)
+    (WTP2: type_unop uop (typeof_pexpr pe) = OK ty),
+    wt_pexpr (Eunop uop pe ty)
+| wt_Ebinop: forall bop pe1 pe2 ty
+    (WTP1: wt_pexpr pe1)
+    (WTP2: wt_pexpr pe2)
+    (** FIXME: we use a very restrictive type checking for binary operation *)
+    (WTP2: type_binop bop (typeof_pexpr pe1) (typeof_pexpr pe2) = OK ty),
+    wt_pexpr (Ebinop bop pe1 pe2 ty).
+    
+Inductive wt_expr: expr -> Prop :=
+| wt_move_place: forall p
+    (WT1: wt_place p)
+    (SCALAR: scalar_type (typeof_place p) = false),
+    wt_expr (Emoveplace p (typeof_place p))
+| wt_pure_expr: forall pe
+    (SCALAR: scalar_type (typeof_pexpr pe) = true)
+    (WT1: wt_pexpr pe),
+    wt_expr pe
+.
+
+
+Inductive wt_stmt: statement -> Prop :=
+| wt_Sassign: forall p e
+    (WT1: wt_place p)
+    (WT2: wt_expr e),
+    (* Require the type of p equal to the type of e? *)
+    wt_stmt (Sassign p e)
+| wt_Sassign_variant: forall p id fid e co
+    (WT1: wt_place p)
+    (WT2: wt_expr e)
+    (WT3: ce ! id = Some co)
+    (* used to prove assign_loc_variant_sound *)
+    (WT4: co.(co_sv) = TaggedUnion),
+    wt_stmt (Sassign_variant p id fid e)
+| wt_Sbox: forall p e ty
+    (WT1: wt_place p)
+    (WT2: wt_expr e)
+    (WT3: typeof_place p = Tbox ty)
+    (* used to prove wt_fooprint *)
+    (SZEQ: sizeof ce ty = sizeof ce (typeof e))
+    (SZCK: 0 < sizeof ce (typeof e) <= Ptrofs.max_unsigned),
+    wt_stmt (Sbox p e)
+.
+    
+(* Well-typed continuation and state *)
+
+Inductive wt_cont: cont -> Prop :=
+| wt_Kseq: forall s k
+    (WT1: wt_stmt s)
+    (WT2: wt_cont k),
+    wt_cont (Kseq s k).
+
+End TYPING.
+
+Coercion env_to_tenv (e: env) : typenv :=
+  PTree.map1 snd e.
+
+Inductive wt_state (ce: composite_env) : state -> Prop :=
+| wt_regular_state: forall f s k (e: env) own m
+    (WT1: wt_stmt e ce s)                  
+    (WT2: wt_cont e ce k),
+    wt_state ce (State f s k e own m)
+| wt_dropplace_state: forall f st drops k own m (e: env)
+    (WT1: Forall (fun p => wt_place e ce p) (map fst drops)),
+    wt_state ce (Dropplace f st drops k e own m)
+.
+
+
+Lemma get_tenv_some: forall e id ty,
+    (env_to_tenv e) ! id = Some ty ->
+    exists b, e ! id = Some (b, ty).
+Proof.
+  intros. unfold env_to_tenv in H. erewrite PTree.gmap1 in H.
+  unfold option_map in H. destruct (e!id) eqn: A; try congruence.
+  destruct p. simpl in H. inv H. eauto.
+Qed.
+
+Lemma sizeof_by_value:
+  forall ce ty chunk,
+  Rusttypes.access_mode ty = Ctypes.By_value chunk -> size_chunk chunk = sizeof ce ty.
+Proof.
+  unfold Rusttypes.access_mode; intros.
+  assert (size_chunk chunk = sizeof ce ty).
+  {
+    destruct ty; try destruct i; try destruct s; try destruct f; inv H; auto;
+    unfold Mptr; simpl; destruct Archi.ptr64; auto.
+  }
+  lia.
+Qed.
+
+Lemma alignof_by_value:
+  forall ce ty chunk,
+  Rusttypes.access_mode ty = Ctypes.By_value chunk -> (align_chunk chunk | alignof ce ty).
+Proof.
+  unfold Rusttypes.access_mode; intros.
+  destruct ty; try destruct i; try destruct s; try destruct f; inv H; auto;
+    unfold Mptr; simpl; destruct Archi.ptr64; try apply Z.divide_refl.
+  exists 2. auto.
+  exists 2. auto.
+Qed.
+
+Lemma wt_place_wt_local: forall p (e: env) ce,
+    wt_place e ce p ->
+    exists b ty, e ! (local_of_place p) = Some (b, ty).
+Proof.
+  induction p; intros.
+  - inv H. simpl. unfold env_to_tenv in WT1. rewrite PTree.gmap1 in WT1.
+    destruct (e!i) eqn: A. inv WT1. destruct p. eauto.
+    inv WT1.
+  - inv H. simpl. eauto.
+  - inv H. simpl. eauto.
+  - inv H. simpl. eauto.
+Qed.
+
+
+(** End of syntactic type checking  *)
