rustfrontend/MoveCheckingDomain.v
@@ -1,0 +1,1281 @@
+Require Import Coqlib .
+Require Import Errors Maps.
+Require Import Values.
+Require Import Integers.
+Require Import AST.
+Require Import Memory.
+Require Import Events.
+Require Import Globalenvs.
+Require Import Smallstep SmallstepLinking SmallstepLinkingSafe.
+Require Import LanguageInterface CKLR Invariant.
+Require Import Rusttypes Rustlight Rustlightown.
+Require Import RustOp RustIR RustIRcfg Rusttyping.
+Require Import Errors.
+Require Import InitDomain InitAnalysis.
+Require Import RustIRown MoveChecking.
+Require Import MoveCheckingFootprint.
+Require Import Wfsimpl.
+
+Import ListNotations.
+
+
+Section COMP_ENV.
+
+Variable ce: composite_env.
+
+(** * Definitions of semantics typedness (TODO: support user-defined semantics types) *)
+
+Definition alignof_comp (id: ident) :=
+  match ce ! id with
+  | Some co => co_alignof co
+  | None => 1
+  end.
+
+(* Semantics well typed location is mutually defined with semantics
+well typed value *)
+Inductive sem_wt_loc (m: mem) : footprint -> block -> Z -> Prop :=
+| sem_wt_base: forall ty b ofs chunk v
+    (MODE: Rusttypes.access_mode ty = Ctypes.By_value chunk)
+    (LOAD: Mem.load chunk m b ofs = Some v)
+    (* (NOTBOX: forall ty', ty <> Tbox ty') *)
+    (WT: sem_wt_val m (fp_scalar ty) v),
+    sem_wt_loc m (fp_scalar ty) b ofs
+| sem_wt_box: forall b ofs fp b1 sz1 v
+    (LOAD: Mem.load Mptr m b ofs = Some v)
+    (WT: sem_wt_val m (fp_box b1 sz1 fp) v),
+    sem_wt_loc m (fp_box b1 sz1 fp) b ofs
+| sem_wt_struct: forall b ofs fpl id
+    (* all fields are semantically well typed *)
+    (FWT: forall fid fofs ffp,
+        find_fields fid fpl = Some (fid, fofs, ffp) ->
+        sem_wt_loc m ffp b (ofs + fofs)),
+    sem_wt_loc m (fp_struct id fpl) b ofs
+| sem_wt_enum: forall fp b ofs tagz fid fofs id orgs
+    (* Interpret the field by the tag and prove that it is well-typed *)
+    (TAG: Mem.load Mint32 m b ofs = Some (Vint (Int.repr tagz)))
+    (FWT: sem_wt_loc m fp b (ofs + fofs)),
+    sem_wt_loc m (fp_enum id orgs tagz fid fofs fp) b ofs
+
+with sem_wt_val (m: mem) : footprint -> val -> Prop :=
+| wt_val_unit:
+  sem_wt_val m (fp_scalar Tunit) (Vint Int.zero)
+| wt_val_int: forall sz si n,
+    (* Cop.cast_int_int sz si n = n -> *)
+    sem_wt_val m (fp_scalar (Tint sz si)) (Vint n)
+| wt_val_single: forall n sz,
+    sem_wt_val m (fp_scalar (Tfloat sz)) (Vsingle n)
+| wt_val_float: forall n sz,
+    sem_wt_val m (fp_scalar (Tfloat sz)) (Vfloat n)
+| wt_val_long: forall si n,
+    sem_wt_val m (fp_scalar (Tlong si)) (Vlong n)
+| wt_val_box: forall b fp sz
+    (** Box pointer must be in the starting point of a block *)
+    (* The value stored in (b,0) has type ty and occupies footprint fp *)
+    (WTLOC: sem_wt_loc m fp b 0)
+    (VALID: Mem.range_perm m b (- size_chunk Mptr) sz Cur Freeable)
+    (SIZE: Mem.load Mptr m b (- size_chunk Mptr) = Some (Vptrofs (Ptrofs.repr sz)))
+    (* sz >0 is used to make sure extcall_ext_free succeeds and sz <=
+    max_unsigned is used to provent overflow when traversing some
+    field offsets *)
+    (RANGE: 0 < sz <= Ptrofs.max_unsigned),
+    sem_wt_val m (fp_box b sz fp) (Vptr b Ptrofs.zero)
+(* TODO *)
+(* | wt_val_ref: forall b ofs ty org mut, *)
+(*     sem_vt_val (Vptr b ofs) (Treference org mut ty) *)
+| wt_val_struct: forall b ofs id fpl
+    (WTLOC: sem_wt_loc m (fp_struct id fpl) b (Ptrofs.unsigned ofs))
+    (AL: (alignof_comp id | Ptrofs.unsigned ofs)),
+    sem_wt_val m (fp_struct id fpl) (Vptr b ofs)
+| wt_val_enum: forall b ofs fp tagz fid fofs id orgs
+    (WTLOC: sem_wt_loc m (fp_enum id orgs tagz fid fofs fp) b (Ptrofs.unsigned ofs))
+    (AL: (alignof_comp id | Ptrofs.unsigned ofs)),
+    sem_wt_val m (fp_enum id orgs tagz fid fofs fp) (Vptr b ofs)
+.
+
+
+Inductive sem_wt_val_list (m: mem) : list footprint -> list val -> Prop :=
+| sem_wt_val_nil:
+  sem_wt_val_list m nil nil
+| sem_wt_val_cons: forall fpl fp vl v,
+    sem_wt_val_list m fpl vl ->
+    sem_wt_val m fp v ->
+    sem_wt_val_list m (fp::fpl) (v::vl)
+.
+
+Inductive bmatch (m: mem) (b: block) (ofs: Z) : footprint -> Prop :=
+| bm_box: forall b1 fp sz
+    (LOAD: Mem.load Mptr m b ofs = Some (Vptr b1 Ptrofs.zero))
+    (SIZE: Mem.load Mptr m b1 (- size_chunk Mptr) = Some (Vptrofs (Ptrofs.repr sz)))
+    (VRES: Mem.range_perm m b1 (- size_chunk Mptr) sz Cur Freeable)
+    (RANGE: 0 < sz <= Ptrofs.max_unsigned),
+    bmatch m b ofs (fp_box b1 sz fp)
+| bm_struct: forall fpl id
+    (* all fields are semantically well typed *)
+    (FMATCH: forall fid fofs ffp,
+        find_fields fid fpl = Some (fid, fofs, ffp) ->
+        bmatch m b (ofs + fofs) ffp),
+    bmatch m b ofs (fp_struct id fpl)
+| bm_enum: forall fp id tagz fid fofs orgs 
+    (* Interpret the field by the tag and prove that it is well-typed *)
+    (* [p] whose value has footprint (fp_enum tagz fp) is actually has
+    tag tagz *)
+    (TAG: Mem.load Mint32 m b ofs = Some (Vint (Int.repr tagz))) 
+    (BM: bmatch m b (ofs + fofs) fp),
+    bmatch m b ofs (fp_enum id orgs tagz fid fofs fp)
+| bm_scalar: forall ty chunk v
+    (* (TY: scalar_type ty = true) *)
+    (MODE: Rusttypes.access_mode ty = Ctypes.By_value chunk)
+    (LOAD: Mem.load chunk m b ofs = Some v)
+    (WT: sem_wt_val m (fp_scalar ty) v),
+    bmatch m b ofs (fp_scalar ty)
+(** TODO: bm_reference  *)
+.
+
+End COMP_ENV.
+
+Global Hint Constructors sem_wt_val sem_wt_loc: sem_ty.
+
+
+(** * Semantics Interface *)
+
+(* Similar to inject_separated: m contains footprint fp1 and fp2 is
+the extended footprint which is not in m *)
+Definition flat_footprint_separated (fp1 fp2: flat_footprint) (m : mem) : Prop :=
+  forall b, ~ In b fp1 ->
+       In b fp2 ->
+       ~ Mem.valid_block m b.
+
+(** Unused because it is equivalent to
+flat_footprint_separated. footprint which not in fp1 and valid in m is
+not in fp2 *)
+Definition flat_footprint_incr (fp1 fp2: flat_footprint) (m: mem) : Prop :=
+  forall b, ~ In b fp1 ->
+       Mem.valid_block m b ->
+       ~ In b fp2.
+  
+Lemma flat_footprint_separated_refl: forall fp m,
+    flat_footprint_separated fp fp m.
+Proof.
+  intros. red. intros. congruence.
+Qed.
+
+(* If the footprint shrinks, the flat_footprint_separated is
+    satisfied trivially *)
+Lemma flat_footprint_separated_shrink: forall l1 l2 m,
+    incl l2 l1 ->
+    flat_footprint_separated l1 l2 m. 
+Proof.
+  intros. red. intros. intro. eapply H0. auto.
+Qed.
+
+Inductive wt_rs_world :=
+  rsw (sg: rust_signature)
+    (fp: flat_footprint)
+    (m: mem)
+    (* used to prove Sbox *)
+    (Hm: Mem.sup_include fp (Mem.support m)).
+
+(** FIXME: we may require that fp is norepet *)
+Inductive wt_rs_query : wt_rs_world -> rust_query -> Prop :=
+| wt_rs_query_intro: forall sg m vf args fpl fp Hm,
+    let ce := rs_sig_comp_env sg in
+    forall (DIS: footprint_disjoint_list fpl)
+    (SEMWT: sem_wt_val_list ce m fpl args)
+    (* footprints are well-typed *)
+    (WTFP: list_forall2 (fun argty fp => wt_footprint (rs_sig_comp_env sg) argty fp) (rs_sig_args sg) fpl)
+    (* structured footprint is equivalent with the flat footprint in the interface *)
+    (EQ: list_equiv fp (flat_map footprint_flat fpl)),
+    wt_rs_query (rsw sg fp m Hm) (rsq vf sg args m)
+.
+
+(* Only consider ownership transfer for now. The footprints of generic
+origins are more complicated *)
+Inductive rsw_acc : wt_rs_world -> wt_rs_world -> Prop :=
+| rsw_acc_intro: forall sg fp fp' m m' Hm Hm'
+    (UNC: Mem.unchanged_on (fun b ofs => ~ In b fp) m m')
+    (* new footprint is separated *)
+    (SEP: flat_footprint_separated fp fp' m),
+    (* block not in fp must be not in fp' otherwise it is not a frame rule *)
+    (* (INCR: flat_footprint_incr fp fp' m), *)
+    rsw_acc (rsw sg fp m Hm) (rsw sg fp' m' Hm').
+
+Inductive wt_rs_reply : wt_rs_world -> rust_reply -> Prop :=
+| wt_rs_reply_intro: forall rfp m rv sg fp Hm,
+    let ce := rs_sig_comp_env sg in
+    forall (SEMWT: sem_wt_val ce m rfp rv)
+    (WTFP: wt_footprint (rs_sig_comp_env sg) (rs_sig_res sg) rfp)
+    (* rfp is separated from fpl *)
+    (SEP: list_disjoint (footprint_flat rfp) fp),
+    wt_rs_reply (rsw sg fp m Hm) (rsr rv m)
+.
+
+Definition wt_rs : invariant li_rs :=
+  {|
+    inv_world := Genv.symtbl * wt_rs_world;
+    symtbl_inv := fun '(se, _) => eq se;
+    query_inv := fun '(_, w) q => wt_rs_query w q;
+    reply_inv := fun '(_, w) r => exists w', rsw_acc w w' /\ wt_rs_reply w' r |}.
+
+
+(* Unused: Rust type used in interface *)
+Inductive rtype : Type :=
+(* primitive types excluding struct and enum *)
+| rt_int (sz: Ctypes.intsize) (sg: Ctypes.signedness)
+| rt_box (ty: rtype)
+| rt_comp
+    (id: ident)
+    (sv: struct_or_variant)
+    (fields: list (ident * rtype))
+    (attr: Ctypes.attr)
+    (orgs: list origin)
+    (rels: list origin_rel)
+(* used in recursive type  *)
+| rt_comp_rec (id: ident)
+.
+
+(* Property of rsw_acc *)
+
+Lemma rsw_acc_refl: forall w,
+    rsw_acc w w.
+Proof.
+  intros. destruct w.
+  econstructor.
+  eapply Mem.unchanged_on_refl.
+  red. intros. congruence.
+Qed.
+  
+Lemma rsw_acc_trans: forall w1 w2 w3,
+    rsw_acc w1 w2 ->
+    rsw_acc w2 w3 ->
+    rsw_acc w1 w3.
+Proof.
+  intros. inv H. inv H0.
+  econstructor.
+  - (* cannot use unchanged_on_trans because fp is not useful in m' *)
+    inv UNC. inv UNC0.
+    econstructor.
+    + eauto with mem.
+    (* perm *)
+    + intros.
+      assert (A: ~ In b fp').
+      { intro. eapply SEP; eauto. }
+      split; intros.
+      * eapply unchanged_on_perm0; eauto.
+        eapply unchanged_on_support; auto.
+        eapply unchanged_on_perm; eauto.
+      * eapply unchanged_on_perm; eauto.
+        eapply unchanged_on_perm0; eauto.
+        eapply Mem.perm_valid_block.
+        eapply unchanged_on_perm0 in H1; eauto.
+        eapply unchanged_on_support. eauto.
+    (* contents *)
+    + intros.
+      assert (A: Mem.valid_block m b).
+      eapply Mem.perm_valid_block. eauto.
+      assert (B: ~ In b fp').
+      { intro. eapply SEP; eauto. }
+      erewrite unchanged_on_contents0; eauto.
+      eapply unchanged_on_perm; eauto.
+  (* flat_footprint_separated *)
+  - red. intros.
+    destruct (Mem.sup_dec b (Mem.support m)); auto.
+    (* impossible *)
+    (* 1. b is in not fp' (by SEP) ; 2. b is in fp'0; 3. so b is not
+    in m' support (by SEP0) *)
+    assert (A: ~ In b fp').
+    { intro. eapply SEP; eauto. }
+    intro. eapply Mem.unchanged_on_support in H1; eauto.
+    eapply SEP0; eauto.
+Qed.    
+
+
+(** * Semantics invariant *)
+
+Section FPM.
+
+Variable fpm : fp_map.
+  
+Definition mmatch ce (m: mem) (e: env) (own: own_env): Prop :=
+  forall p b ofs fp,
+    get_loc_footprint_map e (path_of_place p) fpm = Some (b, ofs, fp) ->
+    is_init own p = true ->
+    bmatch ce m b ofs fp
+    /\ (is_full own.(own_universe) p = true ->
+       sem_wt_loc ce m fp b ofs).
+
+
+Record wf_env (ce: composite_env) (e: env): Prop := {
+    wf_env_footprint: forall id b ty,
+      e!id = Some (b, ty) ->
+      (* Do we need to ensure the location is sem_wt? *)
+      exists fp, fpm!id = Some fp
+            /\ wt_footprint ce ty fp;
+    
+    (* stack blocks and the blocks in footprint map are disjoint. This
+    property can be expressed in sound_state *)
+    (* wf_env_disjoint: *)
+    (* list_disjoint (footprint_of_env e) (flat_fp_map fpm) *)
+    
+  }.
+
+End FPM.
+
+
+(* Some useful invariant of the own_env in the move checking, such as
+if a place p is init, then all its dominators is init. Those
+properties are only guaranteed by the move checking, so we cannot
+prove it in the semantics. One problem is how to establish and
+preserve this invariant in the function entry and every step. May be
+we should do some checking for each function *)
+
+Record wf_own_env le ce (own: own_env) : Prop := {
+    wf_own_dominators: forall p,
+      is_init own p = true ->
+      dominators_is_init own p = true;
+
+    (* validation property *)
+    wf_own_universe_shallow: forall p1 p2,
+      in_universe own p1 = true ->      
+      in_universe own p2 = true ->
+      is_shallow_prefix p1 p2 = false;
+
+    (* all place in the universe has no downcast *)
+    wf_own_no_downcast: forall p fid ty,
+      in_universe own p = true ->
+      ~ In (ph_downcast ty fid) (snd (path_of_place p));
+
+    (* if a place is not full, it must be box type. Remember that if a
+    struct/or some other scalar place is in the universe, it must be
+    full. *)
+    wf_own_type: forall p,
+      in_universe own p = true ->
+      is_full (own_universe own) p = false ->
+      exists ty, typeof_place p = Tbox ty;
+
+    (* all the places in the universe is wt_place *)
+    wf_own_wt_place: forall p,
+      in_universe own p = true ->
+      wt_place le ce p;
+  }.
+
+(* easy because none of the property in wf_own_env rely on some place
+in init set *)
+Lemma wf_own_env_move_place: forall own p le ce,
+    wf_own_env le ce own ->
+    wf_own_env le ce (move_place own p).
+Admitted.
+
+Lemma wf_own_env_init_place: forall own p le ce,
+    dominators_is_init own p = true ->
+    wf_own_env le ce own ->
+    wf_own_env le ce (init_place own p).
+Admitted.
+
+Lemma dominators_is_init_field: forall own p fid fty,
+    dominators_is_init own (Pfield p fid fty) = true ->
+    dominators_is_init own p = true.
+Proof.
+  intros. unfold dominators_is_init in *. simpl in H. auto.
+Qed.
+
+
+(** well-founded relation of composite env *)
+
+Definition ce_extends (env env': composite_env) : Prop := forall id co, env!id = Some co -> env'!id = Some co.
+
+Lemma ce_extends_remove: forall ce1 ce2 id,
+    ce_extends ce1 ce2 ->
+    ce_extends (PTree.remove id ce1) ce2.
+Proof.
+  intros. red.  
+  intros. destruct (ident_eq id id0). subst.
+  rewrite PTree.grs in H0. inv H0.
+  rewrite PTree.gro in H0; eauto.
+Qed.
+
+
+Section COMP_ENV.
+
+Variable ce: composite_env.
+
+(* Lemma downcaset_dominators_eq: forall p fid fty, *)
+(*     place_dominators p = place_dominators (Pdowncast p fid fty). *)
+(* Proof. *)
+(*   induction p; intros; simpl; auto. *)
+
+Inductive valid_owner_offset_footprint : place -> Z -> footprint -> footprint -> Prop :=
+| valid_owner_local: forall id ty fp,
+    valid_owner_offset_footprint (Plocal id ty) 0 fp fp
+| valid_owner_deref: forall p ty fp,
+    valid_owner_offset_footprint (Pderef p ty) 0 fp fp
+| valid_owner_field: forall p fty fid fp,
+    valid_owner_offset_footprint (Pfield p fid fty) 0 fp fp
+| valid_owner_downcast: forall p fid fty fp fp1 tagz fofs ofs id orgs
+    (PTY: typeof_place p = Tvariant orgs id)
+    (* (CO: ce ! id = Some co) *)
+    (* (FOFS: variant_field_offset ce fid co.(co_members) = OK fofs) *)
+    (* (TAG: field_tag fid co.(co_members) = Some tagz) *)
+    (VOWN: valid_owner_offset_footprint p ofs (fp_enum id orgs tagz fid fofs fp) fp1),
+    valid_owner_offset_footprint (Pdowncast p fid fty) (ofs + fofs) fp fp1.
+
+Lemma valid_owner_footprint_flat_eq: forall fp1 fp2 p ofs,
+    valid_owner_offset_footprint p ofs fp1 fp2 ->
+    footprint_flat fp1 = footprint_flat fp2.
+Proof.
+  induction 1; auto.
+Qed.
+
+
+(** So adhoc soluation: define a non-sense valid_owner_offset_footprint to prove the following two lemmas *)
+Lemma valid_owner_place_footprint: forall p fpm e b ofs fp
+    (PFP: get_loc_footprint_map e (path_of_place p) fpm = Some (b, ofs, fp))
+    (WT: wt_place e ce p),
+  exists fp' ofs' fofs,
+    get_loc_footprint_map e (path_of_place (valid_owner p)) fpm = Some (b, ofs', fp')
+    /\ valid_owner_offset_footprint p fofs fp fp'
+    /\ ofs = ofs' + fofs.
+(* relationship between fp and fp'? *)
+                          (* get_footprint *)
+Proof.
+  induction p; intros; simpl in *.
+  - exists fp, ofs, 0. repeat apply conj; auto.
+    econstructor. lia.
+  - exists fp, ofs, 0. repeat apply conj; auto.
+    econstructor. lia.
+  - exists fp, ofs, 0. repeat apply conj; auto.
+    econstructor. lia.
+  - destruct (path_of_place p) eqn: POP.
+    eapply get_loc_footprint_map_app_inv in PFP.
+    destruct PFP as (b1 & ofs1 & fp1 & GET1 & GET2).
+    inv WT.
+    exploit IHp; eauto.
+    intros (fp2 & ofs2 & fofs2 & PFP1 & VOFS1 & OFSEQ).
+    simpl in GET2. destruct fp1; try congruence.
+    rewrite WT2 in GET2.
+    destruct ident_eq in GET2; simpl in GET2; try congruence. subst.
+    destruct list_eq_dec in GET2; simpl in GET2; try congruence. subst.
+    destruct ident_eq in GET2; simpl in GET2; try congruence. subst.
+    (* destruct type_eq in GET2; simpl in GET2; try congruence. *)
+    inv GET2.
+    do 3 eexists. repeat apply conj.
+    eauto. econstructor; eauto.    lia.
+    (* ??? use the fact that variant_field_offset is constant to prove *)
+Qed.
+
+Lemma valid_owner_bmatch: forall p m b ofs1 fofs1 fp1 fp,
+    bmatch ce m b ofs1 fp1 ->
+    valid_owner_offset_footprint p fofs1 fp fp1 ->
+    bmatch ce m b (ofs1 + fofs1) fp.
+Proof.
+  induction p; intros; simpl in *; inv H0; try rewrite Z.add_0_r; auto.
+  exploit IHp; eauto. intros.
+  (* rewrite PTY in H0. inv H0. *)
+  inv H0.
+  replace ((ofs1 + (ofs + fofs))) with (ofs1 + ofs + fofs) by lia.
+  auto.
+Qed.
+
+Lemma valid_owner_sem_wt_loc: forall p m b ofs1 fofs1 fp1 fp,
+    sem_wt_loc ce m fp1 b ofs1 ->
+    valid_owner_offset_footprint p fofs1 fp fp1 ->
+    sem_wt_loc ce m fp b (ofs1 + fofs1).
+Proof.
+  induction p; intros; simpl in *; inv H0; try rewrite Z.add_0_r; auto.
+  exploit IHp; eauto. intros.
+  inv H0. simpl in *. try congruence. 
+  replace ((ofs1 + (ofs + fofs))) with (ofs1 + ofs + fofs) by lia.
+  auto.
+Qed.
+      
+(* get_loc_footprint_map can succeed if the place is well-typed, the
+footprint is well-typed and the footprint is well shaped by
+mmatch. This lemma is used in dropplace state soundness. Because there
+is no static analysis result in dropplace, we need to use own_env to
+show p's dominators are init *)
+Lemma get_loc_footprint_map_progress: forall e m p own fpm
+    (MM: mmatch fpm ce m e own)
+    (WFOWN: wf_env fpm ce e)
+    (WT: wt_place (env_to_tenv e) ce p)
+    (POWN: dominators_is_init own p = true)
+    (** No downcast in the places *)
+    (WF: forall fid ty, ~ In (ph_downcast ty fid) (snd (path_of_place p))),
+  exists b ofs fp,
+    get_loc_footprint_map e (path_of_place p) fpm = Some (b, ofs, fp)
+    /\ wt_footprint ce (typeof_place p) fp.
+Proof.
+  induction p; intros.
+  (* Plocal *)
+  - inv WT. exploit get_tenv_some; eauto. intros (b0 & A).    
+    exploit wf_env_footprint; eauto. intros (fp & FP & WTFP).
+    exists b0, 0, fp. repeat apply conj. simpl. rewrite A. rewrite FP. auto.
+    simpl. auto.
+  (* Pfield *)
+  - inv WT.
+    (** TODO: make it a lemma: prove p's dominators are init *)
+    assert (PDOM: dominators_is_init own p = true).
+    { eapply dominators_is_init_field. eauto. }             
+    assert (IHWF: forall (fid : ident) (ty : type),
+               ~ In (ph_downcast ty fid) (snd (path_of_place p))).
+    { intros. intro. eapply WF. simpl. destruct (path_of_place p) eqn: POP. simpl in *.
+      eapply in_app. eauto. }
+    exploit IHp; eauto.        
+    intros (b & ofs & fp & PFP & WTFP).
+    (* exploit field_type_implies_field_tag; eauto. intros (tag & FTAG & TAGN). *)
+    (** Inversion of WTFP *)
+    rewrite WT2 in WTFP. inv WTFP; simpl in *; try congruence.
+    rewrite WT3 in CO. inv CO.
+    exploit WT0; eauto. intros (ffp & fofs & INFPL & FOFS& WTFP1).
+    exists b, (ofs+fofs), ffp. repeat apply conj; auto.
+    (* get_loc_footprint_map *)
+    simpl. destruct (path_of_place p) eqn: POP.
+    eapply get_loc_footprint_map_app. eauto.
+    simpl.  rewrite INFPL. auto.        
+  (* Pderef *)
+  - inv WT.
+    unfold dominators_is_init in POWN. simpl in POWN.
+    eapply andb_true_iff in POWN. destruct POWN as (PINIT & POWN).
+    assert (IHWF: forall (fid : ident) (ty : type),
+               ~ In (ph_downcast ty fid) (snd (path_of_place p))).
+    { intros. intro. eapply WF. simpl. destruct (path_of_place p) eqn: POP. simpl in *.
+      eapply in_app. eauto. }
+    exploit IHp; eauto.
+    intros (b & ofs & fp & PFP & WTFP).
+    exploit MM; eauto. 
+    intros (BM & FULL).
+    destruct (typeof_place p) eqn: PTY; simpl in WT2; try congruence.
+    inv WT2.
+    (* fp must not be fp_emp that is why we need mmatch *)
+    inv WTFP; inv BM; simpl in *; try congruence.
+    exists b0, 0, fp0. repeat apply conj.    
+    (* get_loc_footprint_map *)
+    destruct (path_of_place p) eqn: POP.
+    eapply get_loc_footprint_map_app. eauto.
+    simpl. auto.
+    (* wt_footprint *)
+    simpl. auto.
+  (* Pdowncast: impossible *)
+  - exfalso. eapply WF.
+    simpl. destruct (path_of_place p) eqn: POP. simpl. eapply in_app.
+    right. econstructor. eauto.
+Qed.
+
+(** IMPRTANT TODO: use this lemma to prove eval_place_sound. Think
+about the field type in wt_footprint is correct or not? *)
+Lemma get_wt_place_footprint_wt: forall p fpm e b ofs fp,
+    wf_env fpm ce e ->
+    wt_place e ce p ->
+    get_loc_footprint_map e (path_of_place p) fpm = Some (b, ofs, fp) ->
+    wt_footprint ce (typeof_place p) fp.
+Proof.
+  intros until fp. intros WFENV WTP GFP.
+  destruct (path_of_place p) eqn: POP.
+  simpl in *.
+  destruct (e!i) eqn: A; try congruence.
+  destruct p0.
+  destruct (fpm ! i) eqn: B; try congruence.
+  exploit wf_env_footprint; eauto. intros (fp1 & C1 & C2).
+  rewrite B in C1. inv C1.
+  eapply get_loc_footprint_eq in GFP.
+  eapply get_wt_footprint_wt; eauto.
+  eapply wt_place_wt_path; eauto.
+Qed.
+
+End COMP_ENV.
+
+Lemma maxv:
+  Ptrofs.max_unsigned = 18446744073709551615.
+Proof.
+  unfold Ptrofs.max_unsigned. unfold Ptrofs.modulus. unfold Ptrofs.wordsize.
+  unfold two_power_nat. unfold Wordsize_Ptrofs.wordsize.
+  replace Archi.ptr64 with true by reflexivity. reflexivity.
+Qed.
+
+(* if a place passes must_movable checking, then the location of this
+place is sem_wt_loc. wt_footprint here is used to make sure that the
+footprint of this place (obtained by get_loc_footprint_map) has the
+same structure as its type, which is used to prevent dynamic footprint
+splitting! *)
+
+Lemma movable_place_sem_wt: forall ce ce1 fp fpm m e own p b ofs init uninit universe
+    (MM: mmatch fpm ce m e own)
+    (POWN: must_movable ce1 init uninit universe p = true)
+    (SOUND: sound_own own init uninit universe)
+    (PFP: get_loc_footprint_map e (path_of_place p) fpm = Some (b, ofs, fp))
+    (WTFP: wt_footprint ce (typeof_place p) fp)
+    (EXTEND: ce_extends ce1 ce),
+    sem_wt_loc ce m fp b ofs.
+Proof.
+  intros ce. intros c. pattern c. apply well_founded_ind with (R := removeR).
+  eapply well_founded_removeR.
+  intros ce1 IH. intros. unfold must_movable, must_movable_fix in *.
+  erewrite unroll_Fix in *.
+  destruct (typeof_place p) eqn: PTY; simpl in POWN; try congruence.
+  - exploit MM. eauto. eapply must_init_sound; eauto.
+    intros (BM & FULL). inv WTFP; inv BM.
+    econstructor; eauto.
+  - exploit MM. eauto. eapply must_init_sound; eauto.
+    intros (BM & FULL). inv WTFP; inv BM.
+    econstructor; eauto.
+  - exploit MM. eauto. eapply must_init_sound; eauto.
+    intros (BM & FULL). inv WTFP; inv BM.
+    econstructor; eauto.
+  - exploit MM. eauto. eapply must_init_sound; eauto.
+    intros (BM & FULL). inv WTFP; inv BM.
+    econstructor; eauto.
+  (* Tbox *)
+  - destruct (must_init init uninit universe p) eqn: INIT; try congruence.
+    destruct (is_full universe p) eqn: PFULL.
+    (* p is full: it must be sem_wt *)
+    eapply MM. eauto. eapply must_init_sound; eauto.
+    erewrite <- is_full_same; eauto. eapply sound_own_universe. eauto.    
+    (* adhoc generalization *)
+    clear PFULL.
+    generalize dependent p. generalize dependent b.
+    generalize dependent fp. generalize dependent ofs.
+    induction t; intros; simpl in *; try congruence.
+    + exploit MM. eauto. eapply must_init_sound; eauto.
+      intros (BM & WTLOC). inv WTFP; inv BM; simpl in *; try congruence.
+      econstructor. eauto.
+      econstructor; eauto.
+      assert (PFP1: get_loc_footprint_map e (path_of_place (Pderef p Tunit)) fpm = Some (b0, 0, fp0)).
+      { simpl. destruct (path_of_place p) eqn: POP.
+        eapply get_loc_footprint_map_app; eauto. }
+      exploit MM. eauto. eapply must_init_sound; eauto.
+      intros (BM1 & WTLOC1). inv WT; inv BM1; simpl in *; try congruence.
+      econstructor; simpl; eauto.
+    (* The same as Tunit case (just copying) *)
+    + exploit MM. eauto. eapply must_init_sound; eauto.
+      intros (BM & WTLOC). inv WTFP; inv BM; simpl in *; try congruence.
+      econstructor. eauto.
+      econstructor; eauto.
+      assert (PFP1: get_loc_footprint_map e (path_of_place (Pderef p (Tint i s))) fpm = Some (b0, 0, fp0)).
+      { simpl. destruct (path_of_place p) eqn: POP.
+        eapply get_loc_footprint_map_app; eauto. }
+      exploit MM. eauto. eapply must_init_sound; eauto.
+      intros (BM1 & WTLOC1). inv WT; inv BM1; simpl in *; try congruence.
+      econstructor; simpl; eauto.
+    + exploit MM. eauto. eapply must_init_sound; eauto.
+      intros (BM & WTLOC). inv WTFP; inv BM; simpl in *; try congruence.
+      econstructor. eauto.
+      econstructor; eauto.
+      assert (PFP1: get_loc_footprint_map e (path_of_place (Pderef p (Tlong s))) fpm = Some (b0, 0, fp0)).
+      { simpl. destruct (path_of_place p) eqn: POP.
+        eapply get_loc_footprint_map_app; eauto. }
+      exploit MM. eauto. eapply must_init_sound; eauto.
+      intros (BM1 & WTLOC1). inv WT; inv BM1; simpl in *; try congruence.
+      econstructor; simpl; eauto.
+    + exploit MM. eauto. eapply must_init_sound; eauto.
+      intros (BM & WTLOC). inv WTFP; inv BM; simpl in *; try congruence.
+      econstructor. eauto.
+      econstructor; eauto.
+      assert (PFP1: get_loc_footprint_map e (path_of_place (Pderef p (Tfloat f))) fpm = Some (b0, 0, fp0)).
+      { simpl. destruct (path_of_place p) eqn: POP.
+        eapply get_loc_footprint_map_app; eauto. }
+      exploit MM. eauto. eapply must_init_sound; eauto.
+      intros (BM1 & WTLOC1). inv WT; inv BM1; simpl in *; try congruence.
+      econstructor; simpl; eauto.
+    (* Induction case *)
+    + destruct (must_init init uninit universe (Pderef p (Tbox t))) eqn: INIT2; try congruence.
+      destruct (is_full universe (Pderef p (Tbox t))) eqn: PFULL1.
+      (* case1: deref p is full: it must be sem_wt *)
+      exploit MM. eauto. eapply must_init_sound; eauto.
+      intros (BM & FULL). inv WTFP; inv BM; simpl in *; try congruence.
+      econstructor; eauto. econstructor; eauto.
+      destruct (path_of_place p) eqn: POP.
+      eapply MM. instantiate (1 := Pderef p (Tbox t)).
+      simpl. rewrite POP. erewrite get_loc_footprint_map_app. eauto.
+      eauto. simpl. auto.
+      eapply must_init_sound; eauto.
+      erewrite <- is_full_same; eauto. eapply sound_own_universe. eauto.
+      (* case2: deref p is not full *)      
+      exploit MM. eauto. eapply must_init_sound; eauto.
+      intros (BM & FULL). inv WTFP; inv BM; simpl in *; try congruence.
+      econstructor. simpl. eauto. eauto.
+      econstructor; eauto.
+      eapply IHt; eauto. simpl. auto.
+      (* get_loc_footprint_map *)
+      simpl. destruct (path_of_place p) eqn: POP.
+      eapply get_loc_footprint_map_app; eauto.
+    (* Tstruct *)
+    + destruct (get_composite ce1 i) eqn: GCO; try congruence. subst.
+      (* fp is not empty *)
+      exploit MM. eauto. eapply must_init_sound; eauto.
+      intros (BM & WTLOC). inv WTFP; inv BM; simpl in *; try congruence.
+      clear GCO. generalize P as P1. intros P1. eapply EXTEND in P. rewrite P in *.
+      econstructor. simpl. eauto. eauto. econstructor; eauto.
+      (* two cases *)
+      destruct (must_init init uninit universe (Pderef p (Tstruct l id1))) eqn: INIT1; try congruence.
+      (** Case1 check that p is full so we can derive sem_wt_loc by mmatch *)
+      destruct (is_full universe (Pderef p (Tstruct l id1))) eqn: FULL; try congruence.
+      (* construct footprint of Pderef p to use mmatch *)
+      assert (PFP1: get_loc_footprint_map e (path_of_place (Pderef p (Tstruct l id1))) fpm = Some (b0, 0, fp0)).
+      { simpl. destruct (path_of_place p) eqn: POP.
+        eapply get_loc_footprint_map_app; eauto. }
+      exploit MM. eauto. eapply must_init_sound; eauto.
+      intros (BM1 & WTLOC1). simpl in *.
+      (* prove sem_wt_loc: first eliminate Tbox *)
+      eapply WTLOC1.
+      erewrite <- is_full_same. eauto. eapply sound_own_universe; eauto.
+      eauto.
+      (** Case2: p is not in the universe *)
+      erewrite forallb_forall in POWN.
+      (** Get the structure of fp by wt_footprint *)
+      inv WT; simpl in *; try congruence. 
+      eapply sem_wt_struct. intros.
+      (* replace fty with (typeof_place (Pfield (Pderef p (Tstruct l id1)) fid fty)) by auto. *)
+      (* strengthen the wt_footprint of struct to require that all
+    element in fpl is in the composite members *)
+      exploit WT2; eauto. intros (fty & A & B & C).
+      eapply IH. instantiate (1 := (PTree.remove id1 ce1)).
+      eapply PTree_removeR. eauto. eauto.
+      assert (INMEM: In (Pfield (Pderef p (Tstruct l id1)) fid fty, fty) (map (fun '(Member_plain fid fty) => (Pfield (Pderef p (Tstruct l id1)) fid fty, fty)) (co_members co))).
+      { exploit field_type_implies_field_tag. eapply A.
+        intros (tag & FTAG & NTH). eapply list_nth_z_in in NTH.
+        eapply in_map_iff. exists (Member_plain fid fty).
+        rewrite  P in CO. inv CO.
+        split; eauto. }
+      generalize (POWN (Pfield (Pderef p (Tstruct l id1)) fid fty, fty) INMEM).
+      instantiate (1 := Pfield (Pderef p (Tstruct l id1)) fid fty).
+      eauto.
+      auto.
+      (* get_loc_footprint_map *)
+      simpl. destruct (path_of_place p) eqn: POP.
+      eapply get_loc_footprint_map_app; eauto.
+      eapply get_loc_footprint_map_app; eauto.
+      simpl. eauto. simpl. rewrite H. auto.
+      (* wt_footprint *)
+      simpl. auto.
+      (* ce_extend *)
+      eapply ce_extends_remove. auto.
+    (* Tvariant *)
+    + destruct (ce1 ! i) eqn: CO; try congruence.      
+      eapply andb_true_iff in POWN. destruct POWN as (INIT1 & FULL).
+      exploit MM. eauto. eapply must_init_sound; eauto.
+      intros (BM & WTLOC). (* rewrite PTY in *. *)
+      inv WTFP; inv BM; simpl in *; try congruence.
+      eapply EXTEND in CO. rewrite CO in *.      
+      econstructor; eauto. 
+      econstructor; eauto.
+      cut (is_full own.(own_universe) (Pderef p (Tvariant l i)) = true).
+      eapply MM.
+      simpl. destruct (path_of_place p) eqn: POP.
+      eapply get_loc_footprint_map_app; eauto.      
+      eapply must_init_sound; eauto.
+      erewrite <- is_full_same; eauto.
+      eapply sound_own_universe; eauto.      
+  (* Tstruct *)
+  - destruct (get_composite ce1 i) eqn: GCO; try congruence. subst.
+    destruct (must_init init uninit universe p) eqn: INIT; try congruence.
+    (** Case1 check that p is full so we can derive sem_wt_loc by mmatch *)
+    destruct (is_full universe p) eqn: FULL; try congruence.
+    exploit MM. eauto. eapply must_init_sound; eauto.
+    intros (BM & WTLOC).  eapply WTLOC.
+    erewrite <- is_full_same. eauto. eapply sound_own_universe; eauto.
+    (** Case2: p is not in the universe *)
+    erewrite forallb_forall in POWN.
+    (** Get the structure of fp by wt_footprint *)
+    inv WTFP; simpl in *; try congruence.
+    eapply sem_wt_struct. intros.
+    (* strengthen the wt_footprint of struct to require that all
+    element in fpl is in the composite members *)
+    exploit WT2; eauto. intros (fty & A & B & C).
+    eapply IH. instantiate (1 := (PTree.remove id1 ce1)).
+    eapply PTree_removeR. eauto. eauto.
+    assert (INMEM: In (Pfield p fid fty, fty) (map (fun '(Member_plain fid fty) => (Pfield p fid fty, fty)) (co_members co))).
+    { exploit field_type_implies_field_tag. eapply A.
+      intros (tag & FTAG & NTH). eapply list_nth_z_in in NTH.
+      eapply in_map_iff. exists (Member_plain fid fty).
+      generalize P as P1. intros. eapply EXTEND in P1.
+      rewrite P1 in CO. inv CO.
+      split; eauto. }    
+    generalize (POWN (Pfield p fid fty, fty) INMEM).
+    instantiate (1 := (Pfield p fid fty)). eauto.    
+    auto.
+    (* place_footprint *)
+    simpl. destruct (path_of_place p) eqn: POP.
+    eapply get_loc_footprint_map_app; eauto.
+    simpl. rewrite H. auto.
+    (* wt_footprint *)
+    simpl. auto.
+    (* ce_extend *)
+    eapply ce_extends_remove; eauto.
+  (* Tvariant *)
+  - destruct (ce1 ! i) eqn: CO; try congruence.
+    eapply andb_true_iff in POWN. destruct POWN as (INIT & FULL).
+    exploit MM. eauto. eapply must_init_sound; eauto.
+    intros (BM & WTLOC). 
+    inv WTFP; inv BM; simpl in *; try congruence. 
+    eapply WTLOC.
+    erewrite <- is_full_same; eauto.
+    eapply sound_own_universe; eauto.
+Qed.
+
+(* properties of place_dominator *)
+
+Lemma place_dominator_local: forall p p',
+    place_dominator p = Some p' ->
+    local_of_place p = local_of_place p'.
+Proof.
+  induction p; simpl; auto.
+  congruence.
+  intros. inv H. auto.
+  intros. inv H. auto.
+Qed.
+
+Lemma place_dominator_strict_prefix: forall p p',
+    place_dominator p = Some p' ->
+    is_prefix_strict p' p = true.
+Proof.
+  induction p; simpl; auto; try congruence; intros.
+  - exploit IHp. eauto. intros A. eapply is_prefix_strict_trans. eauto.
+    eapply is_prefix_strict_field.
+  - inv H. eapply is_prefix_strict_deref.
+  - inv H. eapply is_prefix_strict_downcast.
+Qed.
+
+
+(** Definition of shallow prefix path *)
+
+Lemma move_place_init_is_init: forall p p1 own,
+    is_init (move_place own p1) p = true ->
+    is_init own p = true.
+Admitted.
+
+Lemma move_children_still_init: forall own p1 p2 p3,
+    is_init (move_place own p1) p3 = true ->
+    is_prefix p1 p2 = true ->
+    is_init (move_place own p2) p3 = true.
+Admitted.
+
+Lemma place_dominators_valid_owner_incl: forall p,
+    incl (place_dominators (valid_owner p)) (place_dominators p).
+Proof.
+  induction p; simpl; auto; try apply incl_refl.
+  - red. intros. simpl. right. auto.
+Qed.
+
+Lemma place_dominators_downcast_incl: forall p fid fty,
+    incl (place_dominators p) (place_dominators (Pdowncast p fid fty)).
+Proof.
+  induction p; simpl; auto; intros; try apply incl_nil_l.
+  - red. intros. simpl. right; auto.
+  - red. intros. simpl. right; auto.
+  - apply incl_refl.
+Qed.
+  
+(* what if move out a downcast? Use place_dominators_valid_owner_incl
+and place_dominators_downcast_incl ! *)
+Lemma move_place_dominator_still_init: forall p own,    
+    dominators_is_init own p = true ->
+    dominators_is_init (move_place own p) p = true.
+Proof.
+  induction p; intros; unfold dominators_is_init in *; auto.
+  - simpl in H. 
+    exploit IHp.
+    eauto. intros.
+    eapply forallb_forall. intros.
+    eapply forallb_forall in H0. 2: eauto.
+    eapply move_children_still_init. eauto.
+    eapply is_prefix_field.
+  - simpl in H.
+    eapply andb_true_iff in H. destruct H.
+    exploit IHp.
+    eauto. intros.
+    eapply forallb_forall. intros.
+    simpl in H2. destruct H2; subst.
+    (* case1 *)
+    eapply move_irrelavent_place_still_owned. auto.
+    eapply is_prefix_antisym. eapply is_prefix_strict_deref.
+    (* case2 *)
+    eapply forallb_forall in H1. 2: eauto.
+    eapply move_children_still_init. eauto.
+    eapply is_prefix_deref.
+  - exploit IHp. 
+    (* H can imply the premise of IHp *)
+    eapply forallb_forall. intros.
+    eapply forallb_forall in H. eauto. eapply place_dominators_downcast_incl. auto.
+    intros A.
+    (* valid_owner p is init *)
+    simpl in H.  eapply andb_true_iff in H. destruct H.
+    simpl. eapply andb_true_iff. split.
+    eapply move_irrelavent_place_still_owned. eauto.
+    eapply is_prefix_antisym.
+    eapply is_prefix_strict_trans_prefix2. eapply is_prefix_valid_owner.
+    eapply is_prefix_strict_downcast.
+    (* p's dominators are init so the dominators of (valid_owner p) are init *)
+    eapply forallb_forall. intros.
+    eapply forallb_forall in A. eapply move_children_still_init. eauto.
+    eapply is_prefix_downcast.
+    eapply place_dominators_valid_owner_incl. auto.
+Qed.
+
+  
+(* Inductive not_shallow_prefix_paths: list path -> Prop := *)
+(* | not_shallow_prefix_paths1: forall phs, *)
+(*     not_shallow_prefix_paths (ph_deref :: phs) *)
+(* | not_shallow_prefix_paths2: forall phs ph, *)
+(*     not_shallow_prefix_paths phs -> *)
+(*     not_shallow_prefix_paths (ph :: phs). *)
+
+Definition not_shallow_prefix_paths (phl: list path) : Prop :=
+  In ph_deref phl.
+
+(* Set [vfp] to the path [phl] of [fp1], if [phl] is not shallow paths
+which means that if contains dereference, then [fp2] is still
+bmatch *)
+Lemma bmatch_set_not_shallow_paths: forall phl m b ofs fp1 fp2 vfp ce,
+    bmatch ce m b ofs fp1 ->
+    set_footprint phl vfp fp1 = Some fp2 ->
+    not_shallow_prefix_paths phl ->
+    bmatch ce m b ofs fp2.
+Proof.
+  induction phl; intros; simpl in *; try congruence.
+  red in H1. inv H1.
+  red in H1. inv H1.
+  - destruct fp1; try congruence.
+    destruct (set_footprint phl vfp fp1); try congruence. inv H0.
+    inv H. econstructor; eauto.
+  - destruct a; try congruence.
+    + destruct fp1; try congruence.
+      destruct (set_footprint phl vfp fp1) eqn: A; try congruence.      
+      inv H0. inv H. econstructor; eauto.
+    + destruct fp1; try congruence.
+      destruct (find_fields fid fpl) eqn: A; try congruence.
+      repeat destruct p.
+      exploit find_fields_some. eapply A.
+      intros (B1 & B2). subst.
+      destruct (set_footprint phl vfp f) eqn: B; try congruence.
+      inv H0. inv H. econstructor.
+      intros.            
+      exploit find_fields_some. eauto. intros (C1 & C2).
+      destruct (ident_eq fid i).
+      * subst. erewrite find_fields_set_spec in H; eauto.
+        inv H. destruct peq; try congruence.
+        eapply IHphl; eauto.
+      * eapply FMATCH.
+        eapply find_fields_different_field with (fid:=fid) (id:= i); eauto. 
+    + destruct fp1; try congruence.
+      destruct ty; try congruence.
+      destruct (ident_eq i id) in H0; try congruence; subst.
+      destruct (list_eq_dec ident_eq l orgs) in H0; try congruence; subst.
+      destruct (ident_eq fid fid0) in H0; try congruence; subst.
+      destruct (set_footprint phl vfp fp1) eqn: S in H0; try congruence.
+      inv H0. inv H.
+      econstructor; eauto.
+Qed.
+      
+Lemma not_nil_app_end {A: Type} : forall (l: list A),
+    l <> nil ->
+    exists a l', l = l' ++ [a].
+Proof.
+  induction l. congruence.
+  intros. destruct l.
+  exists a, nil. eauto.
+  exploit IHl; eauto. congruence.
+  intros (a1 & l' & A1). exists a1, (a::l'). rewrite A1. auto.
+Qed.
+
+
+Lemma paths_contain_is_shallow: forall l1 l2,
+    paths_contain l1 (l1 ++ l2) = true ->
+    is_shallow_prefix_paths l2 = true ->
+    paths_shallow_contain l1 (l1 ++ l2) = true.
+Proof.
+  induction l1; intros; simpl in *. auto.
+  destruct path_eq; try congruence. eauto.
+Qed.
+  
+Lemma path_of_not_shallow_prefix: forall p1 p2 l1 l2 id
+    (NSHA: is_shallow_prefix p1 p2 = false)
+    (* is_prefix here is used to avoid syntatic well-typedness *)
+    (PRE: is_prefix p1 p2 = true)
+    (POP1: path_of_place p1 = (id, l1))
+    (POP2: path_of_place p2 = (id, l1 ++ l2)),
+    not_shallow_prefix_paths l2.
+Proof.
+  intros.
+  unfold is_shallow_prefix in NSHA. 
+  unfold is_prefix in PRE.
+  rewrite POP1 in *. rewrite POP2 in *.
+  destruct ident_eq in *; try congruence; simpl in *.
+  destruct (is_shallow_prefix_paths l2) eqn: A.
+  exploit paths_contain_is_shallow; eauto. congruence.
+  eapply negb_false_iff in A.
+  destruct in_dec in A; simpl in *; try congruence. auto.
+Qed.
+
+Lemma paths_shallow_contain_true_implies: forall l1 l2,
+    paths_shallow_contain l1 (l1 ++ l2) = true ->
+    is_shallow_prefix_paths l2 = true.
+Proof.
+  induction l1; intros; simpl in *. auto.
+  destruct path_eq; try congruence; auto.
+Qed.
+
+Lemma is_shallow_prefix_paths_true: forall l,
+    is_shallow_prefix_paths l = true ->
+    ~ not_shallow_prefix_paths l.
+Proof.
+  intros. unfold is_shallow_prefix_paths in H.
+  eapply negb_true_iff in H. destruct in_dec in H; simpl in *; auto.
+  congruence.
+Qed.
+
+(* If the path contains no deref, then p1 must be shallow prefix of
+p2. This lemma is unused *)
+Lemma path_of_not_shallow_prefix_reverse: forall p1 p2 l1 l2 id
+    (NSHA: not_shallow_prefix_paths l2)
+    (POP1: path_of_place p1 = (id, l1))
+    (POP2: path_of_place p2 = (id, l1 ++ l2)),
+    is_shallow_prefix p1 p2 = false.
+Proof.
+  intros.
+  unfold is_shallow_prefix.
+  rewrite POP1. rewrite POP2.
+  eapply andb_false_iff. right.
+  destruct (paths_shallow_contain l1 (l1 ++ l2)) eqn: A; auto.
+  exploit paths_shallow_contain_true_implies. eauto. intros.
+  exploit is_shallow_prefix_paths_true.  eauto. auto. contradiction.
+Qed.  
+
+(** Setting wt_footprint to footprint map  *)
+
+Lemma name_footprints_set_field_same: forall fpl fid fp,
+    name_footprints (set_field fid fp fpl) = name_footprints fpl.
+Proof.
+  induction fpl; simpl; eauto; intros.
+  destruct a. destruct p. destruct ident_eq; subst.
+  simpl. f_equal. simpl. f_equal. eauto.
+Qed.
+
+Lemma name_footprints_update_same: forall fpl,
+    name_footprints (map (fun '(fid, fofs, ffp) => (fid, fofs, clear_footprint_rec ffp)) fpl) = name_footprints fpl.
+Proof.
+  induction fpl; simpl; eauto; intros.
+  destruct a. destruct p. 
+  f_equal. eauto. 
+Qed.
+
+
+Lemma set_wt_footprint: forall phl ty1 vty ce (WTPH: wt_path ce ty1 phl vty) fp1 vfp fp2,
+    set_footprint phl vfp fp1 = Some fp2 ->
+    wt_footprint ce ty1 fp1 ->
+    (* we should not say that vfp is well typed in ce! *)
+    wt_footprint ce vty vfp ->
+    wt_footprint ce ty1 fp2.
+Proof.
+  induction 1; intros until fp2; intros SET WTFP1 WTFP2.
+  - simpl in *. inv SET. auto.
+  - exploit set_footprint_app_inv; eauto.
+    intros (fp3 & vfp1 & A1 & A2 & A3).
+    simpl in A2. destruct fp3; try congruence.
+    inv A2.
+    exploit get_wt_footprint_wt; eauto. intros B1.
+    inv B1.
+    eapply IHWTPH. eauto. eauto.
+    econstructor. simpl in WP2. inv WP2. auto.
+  - exploit set_footprint_app_inv; eauto.
+    intros (fp3 & vfp1 & A1 & A2 & A3).
+    simpl in A2. destruct fp3; try congruence.
+    destruct (find_fields fid fpl) eqn: FIND; try congruence.
+    repeat destruct p. inv A2.
+    exploit get_wt_footprint_wt; eauto. intros B1.
+    inv B1.
+    eapply IHWTPH. eauto. eauto.
+    (* prove wt_footprint of the struct footprint *)
+    econstructor; eauto.
+    + intros. rewrite WP2 in CO. inv CO.
+      exploit WT1. eauto.
+      intros (ffp & fofs & C1 & C2 & C3).
+      erewrite find_fields_set_spec with (fofs:= fofs) (ffp:= ffp); eauto.
+      destruct peq.
+      * subst. exists vfp, fofs.
+        repeat apply conj; auto.
+        rewrite WP3 in H. inv H. auto.
+      * eauto. 
+    + intros. rewrite WP2 in CO. inv CO.
+      exploit find_fields_some. eapply FIND. intros (C1 & C2). subst.
+      destruct (peq i fid0).
+      * subst.
+        exploit WT2.  eauto. intros (fty & F1 & F2 & F3).
+        erewrite find_fields_set_spec with (fofs:= z) (ffp:= f) in H; eauto.
+        inv H. destruct peq; try congruence. eauto.
+      * exploit find_fields_different_field. eauto. eauto.
+        intros FIND1.
+        exploit WT2.  eauto. intros (fty & F1 & F2 & F3).
+        eauto.
+    + erewrite name_footprints_set_field_same; eauto.
+  - exploit set_footprint_app_inv; eauto.
+    intros (fp3 & vfp1 & A1 & A2 & A3).
+    simpl in A2. destruct fp3; try congruence.
+    destruct ident_eq in A2; try congruence.
+    destruct list_eq_dec in A2; try congruence.
+    destruct ident_eq in A2; try congruence.
+    inv A2.
+    exploit get_wt_footprint_wt; eauto. intros B1. 
+    inv B1. eapply IHWTPH. eauto. auto.
+    econstructor; eauto.
+    rewrite WP2 in CO. inv CO. rewrite WP3 in FTY. inv FTY.
+    auto.
+Qed.
+
+(** IMPORTANT TODO: wf_env remain valid if we set a wt_footprint *)
+Lemma wf_env_set_wt_footprint: forall p fpm1 fpm2 ce e fp
+    (WFENV: wf_env fpm1 ce e)
+    (* how to know the type match the type located in the path of the
+    footprint map? *)
+    (WTFP: wt_footprint ce (typeof_place p) fp)
+    (WTP: wt_place e ce p)
+    (SET: set_footprint_map (path_of_place p) fp fpm1 = Some fpm2),
+    wf_env fpm2 ce e.
+Proof.
+  intros.
+  destruct (path_of_place p) eqn: POP.
+  unfold set_footprint_map in SET.
+  destruct (fpm1 ! i) eqn: A1; try congruence.
+  destruct (set_footprint l fp f) eqn: A2; try congruence.
+  inv SET.
+  constructor. intros. exploit wf_env_footprint; eauto.
+  intros (fp1 & B1 & B2).
+  rewrite PTree.gsspec.
+  destruct peq; subst.
+  - exists f0.
+    rewrite A1 in B1. inv B1.
+    split; auto.
+    (* prove wt_footprint after setting *)
+    eapply set_wt_footprint.
+    eapply wt_place_wt_path; eauto.
+    eauto. auto. auto.
+  - eauto.
+Qed.
+
+
+Lemma find_fields_clear_footprint1: forall fpl fid fofs ffp,
+    find_fields fid fpl = Some (fid, fofs, ffp) ->
+    find_fields fid
+      (map (fun '(fid, fofs, ffp) => (fid, fofs, clear_footprint_rec ffp)) fpl) =
+      Some (fid, fofs, (clear_footprint_rec ffp)).
+Proof.
+  induction fpl; simpl; intros; try congruence.
+  destruct a. destruct p.
+  destruct ident_eq.
+  - subst. inv H. auto.
+  - eauto.
+Qed.
+
+Lemma find_fields_clear_footprint2: forall fpl fid fofs ffp,
+    find_fields fid
+      (map (fun '(fid, fofs, ffp) => (fid, fofs, clear_footprint_rec ffp)) fpl) =
+      Some (fid, fofs, ffp) ->
+    exists ffp', find_fields fid fpl = Some (fid, fofs, ffp')
+            /\ ffp = clear_footprint_rec ffp'.
+Proof.
+  induction fpl; simpl; intros; try congruence.
+  destruct a. destruct p.
+  destruct ident_eq.
+  - subst. inv H. eauto.
+  - eauto.
+Qed.
+
+Lemma wt_footprint_clear: forall fp ce ty,
+    wt_footprint ce ty fp ->
+    wt_footprint ce ty (clear_footprint_rec fp).
+Proof.
+  induction fp using strong_footprint_ind; intros; simpl; auto.
+  - inv H. econstructor. destruct ty; simpl in *; try congruence.
+  - inv H. econstructor. congruence.
+  - inv H0. econstructor; eauto.
+    + intros. exploit WT1; eauto.
+      intros (ffp & fofs & A1 & A2 & A3).
+      exists (clear_footprint_rec ffp), fofs. repeat apply conj; auto.
+      * eapply find_fields_clear_footprint1. eauto.
+      * exploit find_fields_some; eauto.
+        intros (B1 & B2).
+        eapply H; eauto.
+    + intros.
+      exploit find_fields_clear_footprint2; eauto.
+      intros (ffp' & A1 & A2). subst.
+      exploit WT2; eauto.
+      intros (fty & B1 & B2 & B3).
+      exists fty. repeat apply conj; auto.
+      exploit find_fields_some; eauto.
+      intros (C1 & C2).
+      eapply H; eauto.
+    + intros. 
+      erewrite name_footprints_update_same; eauto.
+  - inv H. econstructor. congruence.
+Qed.    
+      
+(* clear some footprint does not affect wf_env *)
+Lemma wf_env_clear_footprint: forall fpm1 fpm2 ce e id phl,
+    wf_env fpm1 ce e ->
+    clear_footprint_map e (id, phl) fpm1 = Some fpm2 ->
+    wf_env fpm2 ce e.
+Proof.
+  intros until phl. intros WF CLR.
+  unfold clear_footprint_map in CLR.
+  destruct (get_loc_footprint_map e (id, phl) fpm1) eqn: A; try congruence.
+  repeat destruct p.
+  unfold set_footprint_map in CLR.
+  destruct (fpm1 ! id) eqn: A1; try congruence.
+  destruct (set_footprint phl (clear_footprint_rec f) f0) eqn: A2; try congruence.
+  inv CLR.
+  constructor. intros. exploit wf_env_footprint; eauto.
+  intros (fp1 & B1 & B2).
+  rewrite PTree.gsspec.
+  destruct peq; subst.
+  - exists f1.
+    rewrite A1 in B1. inv B1.
+    split; auto. 
+    (* prove wt_footprint after setting *)
+    unfold get_loc_footprint_map in A. rewrite H in A. rewrite A1 in A.
+    exploit get_wt_footprint_exists_wt; eauto.
+    eapply get_loc_footprint_eq; eauto.
+    intros (ty1 & T1 & T2).  
+    eapply set_wt_footprint; eauto.
+    (* wt_footprint remain if clear the footprint *)
+    eapply wt_footprint_clear. auto.
+  - eauto.
+Qed.
+
+(* Properties of sem_wt_loc *)
+
+Lemma sem_wt_subpath: forall phl fp1 b1 ofs1 b2 ofs2 fp2 ce m,
+    sem_wt_loc ce m fp1 b1 ofs1 ->
+    get_loc_footprint phl fp1 b1 ofs1 = Some (b2, ofs2, fp2) ->
+    sem_wt_loc ce m fp2 b2 ofs2.
+Proof.
+  induction phl; intros.
+  - simpl in H0. inv H0. auto.
+  - simpl in H0. destruct a.
+    + destruct fp1; try congruence.
+      inv H. inv WT. eapply IHphl; eauto.
+    + destruct fp1; try congruence.
+      inv H.
+      destruct (find_fields fid fpl) eqn: FIND; try congruence.
+      repeat destruct p.
+      exploit find_fields_some; eauto. intros (A & B). subst.      
+      exploit FWT; eauto. 
+    + destruct fp1; try congruence.
+      destruct ty; try congruence.
+      destruct ident_eq in H0; subst; try congruence.
+      destruct list_eq_dec in H0; subst; try congruence.
+      destruct ident_eq in H0; subst; try congruence.
+      inv H. eauto.
+Qed.
+
+Lemma sem_wt_loc_implies_bmatch: forall fp m b ofs ce,
+    sem_wt_loc ce m fp b ofs ->
+    bmatch ce m b ofs fp.
+Proof.
+  induction fp using strong_footprint_ind; intros.
+  - inv H.
+  - inv H. econstructor; eauto.
+  - inv H. inv WT.
+    econstructor; eauto.
+  - inv H0. econstructor.
+    intros.
+    exploit find_fields_some; eauto. intros (A & B).
+    exploit FWT; eauto.
+  - inv H. econstructor; eauto.
+Qed.
