rustfrontend/MoveCheckingFootprint.v
@@ -1,0 +1,2365 @@
+Require Import Coqlib .
+Require Import Errors Maps.
+Require Import Values.
+Require Import Integers.
+Require Import AST.
+Require Import Memory.
+Require Import Events.
+Require Import Globalenvs.
+Require Import Smallstep SmallstepLinking SmallstepLinkingSafe.
+Require Import LanguageInterface CKLR Invariant.
+Require Import Rusttypes Rustlight Rustlightown.
+Require Import RustOp RustIR RustIRcfg Rusttyping.
+Require Import Errors.
+Require Import InitDomain InitAnalysis.
+Require Import RustIRown MoveChecking.
+Require Import Wfsimpl.
+
+Import ListNotations.
+
+(** The abstract domain used in the definition of invariant for
+proving the safety of move checking. In particular, we use footprint
+as the abstract value and fp_frame as the abstract memory. They are
+some kinds of separation algebra, but we do not generalize it for
+now. *)
+
+(** Definition of footprint *)
+
+(* A tree structured footprint (maybe similar to some separation logic
+algebra) *)
+Inductive footprint : Type :=
+| fp_emp                      (* empty footprint *)
+| fp_scalar (ty: type)        (* type must be scalar type  *)
+| fp_box (b: block) (sz: Z) (fp: footprint) (* A heap block storing values that occupy footprint fp *)
+(* (field ident, field type, field offset,field footprint) *)
+| fp_struct (id: ident) (fpl: list (ident * Z * footprint))
+(* orgs are not used for now but it is used to relate to the type *)
+| fp_enum (id: ident) (orgs: list origin) (tag: Z) (fid: ident) (ofs: Z) (fp: footprint)
+.
+(* with field_footprint : Type := *)
+(* | fp_field (fid: ident) (fty: type) (ofs: Z) (fp: footprint). *)
+
+Section FP_IND.
+
+Variable (P: footprint -> Prop)
+  (HPemp: P fp_emp)
+  (HPscalar: forall ty, P (fp_scalar ty))
+  (HPbox: forall (b : block) sz (fp : footprint), P fp -> P (fp_box b sz fp))
+  (HPstruct: forall id fpl, (forall fid ofs fp, In (fid, ofs, fp) fpl -> P fp) -> P (fp_struct id fpl))
+  (HPenum: forall id orgs (tag : Z) fid ofs (fp : footprint), P fp -> P (fp_enum id orgs tag fid ofs fp)).
+
+Fixpoint strong_footprint_ind t: P t.
+Proof.
+  destruct t.
+  - apply HPemp.
+  - apply HPscalar.
+  - eapply HPbox. specialize (strong_footprint_ind t); now subst.
+  - eapply HPstruct. induction fpl.
+    + intros. inv H.
+    + intros. destruct a as ((fid1 & ofs1) & fp1).  simpl in H. destruct H.
+      * specialize (strong_footprint_ind fp1). inv H. apply strong_footprint_ind.
+        (* now subst. *)
+      * apply (IHfpl fid ofs fp H). 
+  - apply HPenum. apply strong_footprint_ind.
+Qed.
+    
+End FP_IND.
+
+(* Footprint used in interface (for now, it is just defined by
+support) *)
+Definition flat_footprint : Type := list block.
+
+(* Function used to flatten a footprint  *)
+Fixpoint footprint_flat (fp: footprint) : flat_footprint :=
+  match fp with
+  | fp_emp => nil
+  | fp_scalar _ => nil
+  | fp_box b _ fp' =>
+      b :: footprint_flat fp'
+  | fp_struct _ fpl =>
+      flat_map (fun '(_, _, fp) => footprint_flat fp) fpl
+  | fp_enum _ _ _ _ _ fp =>
+      footprint_flat fp
+  end.
+
+Definition footprint_disjoint (fp1 fp2: footprint) :=
+  list_disjoint (footprint_flat fp1) (footprint_flat fp2).
+
+Inductive footprint_disjoint_list : list footprint -> Prop :=
+| fp_disjoint_nil: footprint_disjoint_list nil
+| fp_disjoint_cons: forall fp fpl,
+      list_disjoint (footprint_flat fp) (flat_map footprint_flat fpl) ->
+      footprint_disjoint_list fpl ->
+      footprint_disjoint_list (fp::fpl)
+.
+
+(* Definition of footprint map *)
+
+Definition fp_map := PTree.t footprint.
+
+(* A footprint in a function frame *)
+
+Definition flat_fp_map (fpm: fp_map) : flat_footprint :=
+  flat_map (fun elt => footprint_flat (snd elt)) (PTree.elements fpm).
+
+(* Definiton of footprint for stack frames *)
+
+(** Footprint map which records the footprint starting from stack
+blocks (denoted by variable names). It represents the ownership chain
+from a stack block. *)
+
+(* The footprint in a module (similar to continuation) *)
+
+Inductive fp_frame : Type :=
+| fpf_emp
+(* we need to record the footprint of the stack *)
+| fpf_func (e: env) (fpm: fp_map) (fpf: fp_frame)
+(* use this to record the structure of footprint in dropplace state, rfp is the footprint of the place being dropped *)
+| fpf_dropplace (e: env) (fpm: fp_map) (rfp: footprint) (fpf: fp_frame)
+(* record the footprint in a drop glue: fp is the footprint being
+dropped and fpl is the footprint of the members to be dropped *)
+| fpf_drop (fp: footprint) (fpl: list footprint) (fpf: fp_frame)
+.
+
+Definition footprint_of_env (e: env) : flat_footprint :=
+  map (fun elt => fst (snd elt)) (PTree.elements e).
+
+
+Fixpoint flat_fp_frame (fpf: fp_frame) : flat_footprint :=
+  match fpf with
+  | fpf_emp => nil
+  | fpf_func e fpm fpf =>
+      footprint_of_env e ++ flat_fp_map fpm ++ flat_fp_frame fpf
+  | fpf_dropplace e fpm rfp fpf =>
+      footprint_of_env e ++ flat_fp_map fpm ++ footprint_flat rfp ++ flat_fp_frame fpf
+  | fpf_drop fp fpl fpf =>
+      footprint_flat fp ++ flat_map footprint_flat fpl ++ flat_fp_frame fpf
+  end.
+
+Lemma in_footprint_of_env: forall b ty id le,
+    le ! id = Some (b, ty) ->
+    In b (footprint_of_env le).
+Proof.
+  intros. unfold footprint_of_env.
+  eapply in_map_iff.
+  exists (id, (b, ty)). split; auto.
+  eapply PTree.elements_correct. eauto.
+Qed.
+
+Lemma in_footprint_flat_fp_map: forall b fp fpm id,
+    fpm ! id = Some fp ->
+    In b (footprint_flat fp) ->
+    In b (flat_fp_map fpm).
+Proof.
+  intros. unfold flat_fp_map.
+  eapply in_flat_map. exists (id, fp). split; auto.
+  eapply PTree.elements_correct. auto.
+Qed.
+
+(* Try to define new sem_wt *)
+
+Definition find_fields (fid: ident) (fpl: list (ident * Z * footprint)) : option (ident * Z * footprint) :=
+  find (fun '(fid', _, _) => if ident_eq fid fid' then true else false) fpl. 
+
+(* Definition set_field (fid: ident) (vfp: footprint) (fpl: list (ident * Z * footprint)) : list (ident * Z * footprint) := *)
+(*   (map *)
+(*      (fun '(fid2, fofs2, ffp2) => *)
+(*         if ident_eq fid fid2 then (fid2, fofs2, vfp) else (fid2, fofs2, ffp2)) fpl). *)
+
+(* only set the first occurence of fid *)
+Fixpoint set_field (fid: ident) (vfp: footprint) (fpl: list (ident * Z * footprint)) : list (ident * Z * footprint) :=
+  match fpl with
+  | nil => nil
+  | (fid', fofs, ffp) :: fpl' =>
+      if ident_eq fid fid' then
+        (fid, fofs, vfp) :: fpl'
+      else
+        (fid', fofs, ffp) :: (set_field fid vfp fpl')
+  end.
+
+
+Lemma find_fields_some: forall fid fid1 fpl fofs ffp,
+    find_fields fid fpl = Some (fid1, fofs, ffp) ->
+    fid = fid1 /\ In (fid, fofs, ffp) fpl.
+Proof.
+  intros. unfold find_fields in H.
+  exploit find_some; eauto. intros (A & B).
+  destruct ident_eq in B; try congruence.
+  subst. auto.
+Qed.
+
+Lemma find_fields_different_field: forall fpl fid id fofs ffp vfp,
+    id <> fid ->
+    find_fields fid (set_field id vfp fpl) = Some (fid, fofs, ffp) ->
+    find_fields fid fpl = Some (fid, fofs, ffp).
+Proof.
+  induction fpl; intros; simpl in *; try congruence.
+  destruct a. destruct p. destruct ident_eq in H0.
+  - subst. destruct ident_eq.
+    + subst. congruence.
+    + simpl in H0. destruct ident_eq in H0; try congruence.
+  - destruct ident_eq.
+    + subst. simpl in H0. destruct ident_eq in H0; try congruence.
+    + simpl in H0. destruct ident_eq in H0; try congruence.
+      eauto.
+Qed.
+
+Ltac simpl_find_fields :=
+  match goal with
+  | [H :find_fields _ (_ :: _) = Some _ |- _ ] =>
+      simpl; simpl in H;
+      destruct ident_eq; try congruence
+  | [ |- find_fields _ (_ :: _) = Some _ ] =>
+      simpl;
+      destruct ident_eq; try congruence
+  end.
+
+Lemma find_fields_same_offset: forall fpl fid id fofs ffp vfp,
+    find_fields fid (set_field id vfp fpl) = Some (fid, fofs, ffp) ->
+    exists vfp1, find_fields fid fpl = Some (fid, fofs, vfp1).
+Proof.
+  induction fpl; intros; simpl in *; try congruence.
+  destruct a. destruct p. destruct ident_eq in H.
+  - subst. simpl_find_fields.
+    + inv H. eauto.
+    + eauto.
+  - simpl_find_fields.
+    + inv H. eauto.
+    + eauto.
+Qed.
+
+Lemma find_fields_same_footprint: forall fpl fid fofs ffp vfp,
+    find_fields fid (set_field fid vfp fpl) = Some (fid, fofs, ffp) ->
+    vfp = ffp.
+Proof.
+  induction fpl; intros; simpl in *; try congruence.
+  destruct a. destruct p. destruct ident_eq in H.
+  - subst. simpl_find_fields.
+  - simpl_find_fields. eauto.
+Qed.
+
+Lemma find_fields_set_spec: forall fpl fid1 fid2 fofs ffp vfp,
+    find_fields fid1 fpl = Some (fid1, fofs, ffp) ->
+    find_fields fid1 (set_field fid2 vfp fpl) = Some (fid1, fofs, if peq fid1 fid2 then vfp else ffp).
+Proof.
+  induction fpl; intros; simpl in *; try congruence.
+  destruct a. destruct p.
+  destruct ident_eq in H.
+  - subst. inv H. destruct ident_eq; subst.
+    + destruct ident_eq; try congruence.
+      simpl. destruct ident_eq; try congruence.
+      auto.
+    + simpl_find_fields.
+      destruct peq; try congruence. auto.
+  - destruct ident_eq; subst.
+    + simpl_find_fields.
+    + simpl_find_fields. eauto.
+Qed.
+
+Definition name_footprints (fpl: list (ident * Z * footprint)) : list ident :=
+  map (fun '(fid, _, _) => fid) fpl.
+
+Lemma find_fields_split: forall fpl id fofs ffp,
+    find_fields id fpl = Some (id, fofs, ffp) ->
+    exists l1 l2,
+      fpl = l1 ++ (id, fofs, ffp) :: l2
+      /\ ~ In id (name_footprints l1).
+Proof.
+  induction fpl; simpl; intros.
+  - inv H.
+  - destruct a. destruct p.
+    destruct ident_eq.
+    + inv H. exists nil, fpl.
+      split. simpl. auto.
+      intro. inv H.
+    + exploit IHfpl; eauto. intros (l1 & l2 & A1 & A2).
+      subst.
+      exists ((i,z,f)::l1), l2. split; auto.
+      intro. inv H0; congruence. 
+Qed.
+      
+Lemma set_fields_split: forall l1 l2 id fofs ffp ffp1,
+    ~ In id (name_footprints l1) ->
+    set_field id ffp1 (l1 ++ (id, fofs, ffp) :: l2 ) = (l1 ++ (id, fofs, ffp1) :: l2).
+Proof.
+  induction l1; simpl; intros.
+  - destruct ident_eq; try congruence.
+  - destruct a. destruct p. eapply Decidable.not_or in H.
+    destruct H. destruct ident_eq; try congruence.
+    f_equal. eauto.
+Qed.
+
+
+(** Definition of path disjointness in the footprint *)
+
+Inductive paths_disjoint : list path -> list path -> Prop :=
+| phs_disjoint1: forall p1 p2 l1 l2,
+    (* Is it enough to use neq? *)
+    p1 <> p2 ->
+    paths_disjoint (p1::l1) (p2::l2)
+| phs_disjoint2: forall p l1 l2,
+    paths_disjoint l1 l2 ->
+    paths_disjoint (p::l1) (p::l2).
+
+Lemma paths_disjoint_sym: forall phl1 phl2,
+    paths_disjoint phl1 phl2 ->
+    paths_disjoint phl2 phl1.
+Proof.
+  induction 1.
+  econstructor. eauto.
+  eapply phs_disjoint2; auto.
+Qed.
+
+Lemma local_of_paths_of_place: forall p,
+    local_of_place p = fst (path_of_place p).
+Proof.
+  induction p; simpl; auto; destruct (path_of_place p); auto.
+Qed.
+
+
+Lemma paths_not_contain_disjoint: forall l1 l2,
+    paths_contain l1 l2 = false ->
+    paths_contain l2 l1 = false ->
+    paths_disjoint l1 l2.
+Proof.
+  induction l1; intros; simpl in *.
+  - congruence.
+  - destruct l2; simpl in *; try congruence.
+    destruct path_eq; subst; destruct path_eq; try congruence.
+    eapply phs_disjoint2. auto.
+    eapply phs_disjoint1; auto.
+Qed.
+
+Lemma is_not_prefix_disjoint: forall p1 p2,
+    is_prefix p1 p2 = false ->
+    is_prefix p2 p1 = false ->
+    fst (path_of_place p1) <> fst (path_of_place p2) \/
+      paths_disjoint (snd (path_of_place p1)) (snd (path_of_place p2)).
+Proof.
+  intros. unfold is_prefix in *.
+  destruct (path_of_place p1) eqn: POP1.
+  destruct (path_of_place p2) eqn: POP2.  
+  simpl.
+  destruct ident_eq in H; destruct ident_eq in H0; subst;  simpl in *; try congruence; auto.
+  right. eapply paths_not_contain_disjoint; auto.
+Qed.  
+
+Lemma paths_contain_app_inv: forall l1 l2,
+    paths_contain l1 l2 = true ->
+    exists l3, l2 = l1 ++ l3.
+Proof.
+  induction l1; intros; simpl in *; eauto.
+  destruct l2; try congruence; eauto.
+  destruct path_eq; subst; try congruence; eauto.
+  exploit IHl1; eauto. intros (l3 & A1). subst. eauto.
+Qed.
+
+Lemma is_prefix_paths_app: forall p1 p2,
+    is_prefix p1 p2 = true ->
+    fst (path_of_place p1) = fst (path_of_place p2)
+    /\ exists phl, snd (path_of_place p2) = snd (path_of_place p1) ++ phl.
+Proof.
+  intros. destr_prefix.
+  split. auto.
+  eapply paths_contain_app_inv. eauto.
+Qed.
+
+
+(** * Functions and properties for updating the footprint *)
+
+(** Prove some properties w.r.t list_nth_z  *)
+Fixpoint list_set_nth_z {A: Type} (l: list A) (n: Z) (v: A)  {struct l}: list A :=
+  match l with
+  | nil => nil
+  | hd :: tl => if zeq n 0 then (v :: tl) else hd :: (list_set_nth_z tl (Z.pred n) v)
+  end.
+
+(* set footprint [v] in the path [ph] of footprint [fp] *)
+Fixpoint set_footprint (phl: list path) (v: footprint) (fp: footprint) : option footprint :=
+  match phl with
+  | nil => Some v
+  | ph :: l =>
+        match ph, fp with
+        | ph_deref, fp_box b sz fp1 =>
+            match set_footprint l v fp1 with
+            | Some fp2 =>
+                Some (fp_box b sz fp2)
+            | None => None
+            end
+        | ph_field fid, fp_struct id fpl =>
+            match find_fields fid fpl with
+            | Some (fid1, fofs, ffp) =>                
+                match set_footprint l v ffp with
+                | Some ffp1 =>
+                    Some (fp_struct id (set_field fid ffp1 fpl)) 
+                | None => None
+                end
+            | None => None
+            end
+        | ph_downcast pty fid (* fty *), fp_enum id orgs tagz fid1 fofs1 fp1 =>
+            match pty with
+            | Tvariant orgs1 id1 =>
+                if ident_eq id1 id then
+                  if list_eq_dec ident_eq orgs1 orgs then
+                    if ident_eq fid fid1 then
+                      match set_footprint l v fp1 with
+                      | Some fp2 =>
+                          Some (fp_enum id orgs tagz fid1 fofs1 fp2)
+                      | None => None
+                      end
+                    else None
+                  else None
+                else None
+            | _ => None
+            end
+        | _, _ => None
+        end
+  end.
+
+Fixpoint clear_footprint_rec (fp: footprint) : footprint :=
+  match fp with
+  | fp_scalar _
+  | fp_box _ _ _
+  | fp_enum _ _ _ _ _ _
+  | fp_emp => fp_emp
+  | fp_struct id fpl =>
+      fp_struct id (map (fun '(fid, fofs, ffp) => (fid, fofs, clear_footprint_rec ffp)) fpl)
+  end.
+
+Fixpoint get_loc_footprint (phl: list path) (fp: footprint) (b: block) (ofs: Z) : option (block * Z * footprint) :=
+  match phl with
+  | nil => Some (b, ofs, fp)
+  | ph :: l =>
+      match ph, fp with
+      | ph_deref, fp_box b _ fp1 =>
+          get_loc_footprint l fp1 b 0
+      | ph_field fid, fp_struct _ fpl =>
+          match find_fields fid fpl with
+          | Some (_, fofs, fp1) =>
+              get_loc_footprint l fp1 b (ofs + fofs)
+          | None => None
+          end
+      | ph_downcast pty fid1 (* fty1 *), fp_enum id orgs _ fid2 fofs fp1 =>
+          match pty with
+          | Tvariant orgs1 id1 =>
+              if ident_eq id1 id then
+                if list_eq_dec ident_eq orgs1 orgs then
+                if ident_eq fid1 fid2  then
+                  get_loc_footprint l fp1 b (ofs + fofs)
+                else
+                  None
+                else None
+              else None
+          | _ => None
+          end
+      | _, _  => None
+      end
+  end.
+
+(* non-loc version: use it to get some internal footprint *)
+Fixpoint get_footprint (phl: list path) (fp: footprint) : option footprint :=
+  match phl with
+  | nil => Some fp
+  | ph :: l =>
+      match ph, fp with
+      | ph_deref, fp_box b _ fp1 =>
+          get_footprint l fp1
+      | ph_field fid, fp_struct _ fpl =>
+          match find_fields fid fpl with
+          | Some (_, fofs, fp1) =>
+              get_footprint l fp1
+          | None => None
+          end
+      | ph_downcast pty fid1 (* fty1 *), fp_enum id orgs _ fid2 fofs fp1 =>
+          match pty with
+          | Tvariant orgs1 id1 =>
+              if ident_eq id1 id then
+                if list_eq_dec ident_eq orgs1 orgs then
+                  if ident_eq fid1 fid2 then
+                    get_footprint l fp1
+                  else
+                    None
+                else None
+              else None
+          | _ => None
+          end
+      | _, _  => None
+      end
+  end.
+
+
+(* Definition clear_footprint (phl: list path) (fp: footprint) : option footprint := *)
+(*   match get_footprint phl fp with *)
+(*   | Some fp1 => *)
+(*       set_footprint phl (clear_footprint_rec fp1) fp *)
+(*   | None => None *)
+(*   end. *)
+
+
+Definition set_footprint_map (ps: paths) (v: footprint) (fpm: fp_map) : option fp_map :=
+  let (id, phl) := ps in
+  match fpm!id with
+  | Some fp1 =>
+      match set_footprint phl v fp1 with
+      | Some fp2 =>
+          Some (PTree.set id fp2 fpm)
+      | None =>
+          None
+      end
+  | None => None
+  end.
+
+
+Definition get_loc_footprint_map (e: env) (ps: paths) (fpm: fp_map) : option (block * Z * footprint) :=
+  let (id, phl) := ps in
+  match e!id, fpm!id with
+  | Some (b, ty), Some fp =>
+      get_loc_footprint phl fp b 0
+  | _, _ => None
+  end.
+
+
+(* Definition get_footprint_map (ps: paths) (fpm: fp_map) : option footprint := *)
+(*   let (id, phl) := ps in *)
+(*   match fpm!id with *)
+(*   | Some fp => *)
+(*       get_footprint phl fp *)
+(*   | None => None *)
+(*   end. *)
+
+Definition clear_footprint_map e (ps: paths) (fpm: fp_map) : option fp_map :=
+  match get_loc_footprint_map e ps fpm with
+  | Some (_, _, fp1) =>
+      set_footprint_map ps (clear_footprint_rec fp1) fpm
+  | None => None
+  end.
+
+(* Useful tactic to destruct get_loc_footprint *)
+Ltac destr_fp_enum fp ty :=
+  destruct fp; try congruence;
+  destruct ty; try congruence;
+  destruct ident_eq; try congruence;
+  destruct list_eq_dec; try congruence;
+  destruct ident_eq; try congruence; subst.
+
+Ltac destr_fp_field fp H :=
+  let A1 := fresh "A" in
+  let A2 := fresh "A" in
+  let p := fresh "p" in
+  let FIND := fresh "FIND" in
+  destruct fp; try congruence;
+  destruct find_fields as [p|] eqn: FIND; try congruence;
+  repeat destruct p; simpl in H;
+exploit find_fields_some; eauto; intros (A1 & A2); subst.
+
+
+Lemma get_loc_footprint_app: forall phl1 phl2 fp fp1 b ofs b1 ofs1 b2 ofs2 fp2,
+    get_loc_footprint phl1 fp b ofs = Some (b1, ofs1, fp1) ->
+    get_loc_footprint phl2 fp1 b1 ofs1 = Some (b2, ofs2, fp2) ->
+    get_loc_footprint (phl1 ++ phl2) fp b ofs = Some (b2, ofs2, fp2).
+Proof.
+  induction phl1; simpl; intros.
+  - inv H. auto.
+  - destruct a.
+    + destruct fp; try congruence.
+      eauto.
+    + destr_fp_field fp H.
+    + destr_fp_enum fp ty.
+      eauto.
+Qed.
+         
+Lemma get_loc_footprint_map_app: forall phl2 phl1 id e fpm b ofs fp b1 ofs1 fp1,
+    get_loc_footprint_map e (id, phl1) fpm = Some (b, ofs, fp) ->
+    get_loc_footprint phl2 fp b ofs = Some (b1, ofs1, fp1) ->
+    get_loc_footprint_map e (id, phl1 ++ phl2) fpm = Some (b1, ofs1, fp1).
+Proof.
+  induction phl2; intros.
+  - simpl in H0. inv H0. rewrite app_nil_r. auto.
+  - unfold get_loc_footprint_map in H.
+    destruct (e ! id) eqn: ID; try congruence. destruct p.
+    destruct (fpm ! id) eqn: FPM; try congruence.     
+    replace (a :: phl2) with ((a::nil) ++ phl2) by auto.
+    rewrite app_assoc.
+    simpl in H0. destruct a.
+    + destruct fp; try congruence.          
+      eapply IHphl2. 
+      unfold get_loc_footprint_map. rewrite ID. rewrite FPM.
+      eapply get_loc_footprint_app. eauto.
+      simpl. eauto. auto.
+    + destruct fp; try congruence.
+      destruct (find_fields fid fpl) eqn: FIND; try congruence.
+      repeat destruct p.
+      eapply IHphl2. 
+      unfold get_loc_footprint_map. rewrite ID. rewrite FPM.
+      eapply get_loc_footprint_app. eauto.
+      simpl. rewrite FIND. eauto. auto.
+    + destruct fp; try congruence.
+      destruct ty; try congruence. destruct ident_eq in H0; try congruence. subst.
+      destruct list_eq_dec in H0; try congruence.
+      destruct ident_eq in H0; simpl in H0; try congruence. subst.            
+      (* destruct type_eq in H0; simpl in H0; try congruence. subst. *)
+      eapply IHphl2. 
+      unfold get_loc_footprint_map. rewrite ID. rewrite FPM.
+      eapply get_loc_footprint_app. eauto.
+      simpl. destruct ident_eq; simpl; try congruence.
+      destruct ident_eq; simpl; try congruence.
+      destruct list_eq_dec; try congruence.
+      (* destruct type_eq; simpl; try congruence. *)
+      eauto. auto.
+Qed.
+
+
+Lemma get_loc_footprint_app_inv: forall phl1 phl2 b1 b2 ofs1 ofs2 fp1 fp2,
+    get_loc_footprint (phl1 ++ phl2) fp1 b1 ofs1 = Some (b2, ofs2, fp2) ->
+    exists b3 ofs3 fp3,
+      get_loc_footprint phl1 fp1 b1 ofs1 = Some (b3, ofs3, fp3)
+      /\ get_loc_footprint phl2 fp3 b3 ofs3 = Some (b2, ofs2, fp2).
+Proof.
+  induction phl1; intros; simpl in *.
+  - eauto.
+  - destruct a.
+    + destruct fp1; try congruence.
+      eauto.
+    + destruct fp1; try congruence.
+      destruct (find_fields fid fpl) eqn: FIND; try congruence.
+      repeat destruct p.
+      eauto.
+    + destr_fp_enum fp1 ty.
+      eauto.
+Qed.
+
+      
+Lemma get_loc_footprint_map_app_inv: forall phl2 phl1 id e fpm b1 ofs1 fp1,
+    get_loc_footprint_map e (id, phl1 ++ phl2) fpm = Some (b1, ofs1, fp1) ->
+    exists b ofs fp,
+      get_loc_footprint_map e (id, phl1) fpm = Some (b, ofs, fp)
+      /\ get_loc_footprint phl2 fp b ofs = Some (b1, ofs1, fp1).
+Proof.
+  intros. simpl in *.
+  destruct (e!id); try congruence.
+  destruct p.
+  destruct (fpm!id); try congruence.
+  eapply get_loc_footprint_app_inv; eauto.
+Qed.
+
+
+Lemma get_set_footprint_exists: forall phl fp1 fp b ofs b1 ofs1 vfp,
+    get_loc_footprint phl fp b ofs = Some (b1, ofs1, fp1) ->
+    exists fp2, set_footprint phl vfp fp = Some fp2
+           /\ get_loc_footprint phl fp2 b ofs = Some (b1, ofs1, vfp).
+Proof.
+  induction phl; simpl; intros.
+  - inv H. eauto.
+  - destruct a.
+    + destruct fp; try congruence.
+      exploit IHphl; eauto.
+      instantiate (1 := vfp). intros (fp2 & A1 & A2).
+      rewrite A1. eexists. split; eauto.
+    + destruct fp; try congruence.
+      destruct (find_fields fid fpl) eqn: FIND; try congruence.
+      repeat destruct p.
+      exploit IHphl; eauto.
+      instantiate (1 := vfp). intros (fp2 & A1 & A2).
+      rewrite A1.
+      eexists; split; eauto.
+      exploit find_fields_some; eauto. intros (B1 & B2). subst.
+      simpl. erewrite find_fields_set_spec; eauto.
+      destruct peq; try congruence.
+    + destr_fp_enum fp ty.
+      exploit IHphl; eauto.
+      instantiate (1 := vfp). intros (fp2 & A1 & A2).
+      rewrite A1.
+      eexists; split; eauto.
+      simpl. destruct ident_eq; try congruence.
+      destruct list_eq_dec; try congruence.
+      destruct ident_eq; try congruence.
+Qed.
+     
+Lemma get_set_footprint_map_exists: forall phl id fp fp1 fpm1 b ofs le,
+    get_loc_footprint_map le (id, phl) fpm1 = Some (b, ofs, fp1) ->
+    exists fpm2, set_footprint_map (id, phl) fp fpm1 = Some fpm2
+            /\ get_loc_footprint_map le (id, phl) fpm2 = Some (b, ofs, fp).
+Proof.
+  intros. simpl in *.
+  destruct (le ! id) eqn: A; try congruence. destruct p.
+  destruct (fpm1 ! id) eqn: B; try congruence.
+  exploit get_set_footprint_exists; eauto. instantiate (1 := fp).
+  intros (fp2 & A1 & A2). rewrite A1.
+  eexists; split; eauto.
+  rewrite PTree.gss. auto.
+Qed.
+
+Lemma get_set_footprint_app_inv: forall phl1 phl2 fp1 fp2 fp fp' b1 ofs1 b ofs,
+    get_loc_footprint phl1 fp b ofs = Some (b1, ofs1, fp1) ->
+    set_footprint (phl1++phl2) fp2 fp = Some fp' ->
+    exists fp3,
+      get_loc_footprint phl1 fp' b ofs = Some (b1, ofs1, fp3)
+      /\ set_footprint phl2 fp2 fp1 = Some fp3.
+Proof.
+  induction phl1; simpl; intros.
+  - inv H. eauto.
+  - destruct a.
+    + destruct fp; try congruence.
+      destruct (set_footprint (phl1 ++ phl2) fp2 fp) eqn: A; try congruence.
+      inv H0.
+      exploit IHphl1; eauto.
+    + destruct fp; try congruence.
+      destruct (find_fields fid fpl) eqn: FIND; try congruence.
+      repeat destruct p.
+      destruct (set_footprint (phl1 ++ phl2) fp2 f) eqn: A; try congruence.
+      inv H0.
+      exploit find_fields_some; eauto. intros (B1 & B2). subst.
+      erewrite find_fields_set_spec; eauto.
+      destruct peq; try congruence.
+      eauto.
+    + destr_fp_enum fp ty.
+      destruct (set_footprint (phl1 ++ phl2) fp2 fp) eqn: A; try congruence.
+      inv H0.
+      destruct ident_eq; try congruence.
+      destruct list_eq_dec; try congruence.
+      destruct ident_eq; try congruence.
+      eauto.
+Qed.
+      
+Lemma get_set_footprint_map_app_inv: forall phl2 phl1 id fpm1 fpm2 fp1 fp2 b1 ofs1 le,
+    get_loc_footprint_map le (id, phl1) fpm1 = Some (b1, ofs1, fp1) ->
+    set_footprint_map (id, phl1++phl2) fp2 fpm1 = Some fpm2 ->
+    exists fp3,
+      get_loc_footprint_map le (id, phl1) fpm2 = Some (b1, ofs1, fp3)
+      /\ set_footprint phl2 fp2 fp1 = Some fp3.
+Proof.
+  intros. simpl in *.
+  destruct (le!id) eqn: A; try congruence. destruct p.
+  destruct (fpm1!id) eqn: B; try congruence.
+  destruct (set_footprint (phl1 ++ phl2) fp2 f) eqn: C; try congruence.
+  inv H0. rewrite PTree.gss.
+  eapply get_set_footprint_app_inv; eauto.
+Qed.
+
+Lemma set_footprint_app: forall l1 l2 fp1 fp1' fp2 fp fp',
+         get_footprint l1 fp = Some fp1 ->
+        set_footprint l2 fp2 fp1 = Some fp1' ->
+        set_footprint l1 fp1' fp = Some fp' ->
+        set_footprint (l1++l2) fp2 fp = Some fp'.
+Proof.
+  induction l1; intros.
+  - simpl in *. inv H. inv H1. auto.
+  - simpl in *. destruct a.
+    + destruct fp; try congruence.
+      destruct (set_footprint l1 fp1' fp) eqn: A; try congruence.
+      inv H1. erewrite IHl1; eauto.
+    + destruct fp; try congruence.
+      destruct (find_fields fid fpl) eqn: FIND; try congruence.
+      repeat destruct p.
+      destruct (set_footprint l1 fp1' f) eqn: SET; try congruence.
+      inv H1. erewrite IHl1; eauto.
+    + destruct fp; try congruence.
+      destruct ty; try congruence.
+      destruct ident_eq; try congruence.
+      destruct list_eq_dec; try congruence.
+      destruct ident_eq; try congruence.
+      destruct (set_footprint l1 fp1' fp) eqn: SET; try congruence.
+      erewrite IHl1; eauto.
+Qed.
+
+(** IMPORTANT TODO *)
+Lemma set_footprint_app_inv : forall l1 l2 fp fp' vfp1,
+    set_footprint (l1++l2) vfp1 fp = Some fp' ->
+    exists fp'' vfp2,
+      get_footprint l1 fp = Some fp''                                       
+      /\ set_footprint l2 vfp1 fp'' = Some vfp2
+      /\ set_footprint l1 vfp2 fp = Some fp'.
+Proof.
+  induction l1; intros.
+  - simpl in H. exists fp, fp'. simpl.
+    repeat apply conj; auto.
+  - simpl in H. destruct a.
+    + destruct fp; try congruence.
+      destruct (set_footprint (l1 ++ l2) vfp1 fp) eqn: A; try congruence.
+      inv H. exploit IHl1; eauto.
+      intros (fp'' & vfp'2 & B1 & B2 & B3).
+      simpl.
+      exists fp'', vfp'2. repeat apply conj; auto.
+      rewrite B3. auto.
+    + destruct fp; try congruence.
+      destruct (find_fields fid fpl) eqn: FIND; try congruence.
+      repeat destruct p.
+      destruct (set_footprint (l1 ++ l2) vfp1 f) eqn: A; try congruence.
+      inv H. exploit IHl1; eauto.
+      intros (fp'' & vfp'2 & B1 & B2 & B3).
+      simpl. rewrite FIND.
+      exists fp'', vfp'2. repeat apply conj; auto.
+      rewrite B3. auto.
+    + destruct fp; try congruence.
+      destruct ty; try congruence.
+      simpl.
+      destruct ident_eq; try congruence.
+      destruct list_eq_dec; try congruence.
+      destruct ident_eq; try congruence.
+      destruct (set_footprint (l1 ++ l2) vfp1 fp) eqn: A; try congruence.
+      inv H. exploit IHl1; eauto.
+      intros (fp'' & vfp'2 & B1 & B2 & B3).
+      simpl.      
+      exists fp'', vfp'2. repeat apply conj; auto.
+      rewrite B3. auto.
+Qed.
+
+      
+(* non-loc version of get_footprint_app *)
+Lemma get_footprint_app: forall l1 l2 fp1 fp2 fp3,
+    get_footprint l1 fp1 = Some fp2 ->
+    get_footprint l2 fp2 = Some fp3 ->
+    get_footprint (l1 ++ l2) fp1 = Some fp3.
+Proof.
+  induction l1; intros; simpl in *.
+  - inv H. auto.
+  - destruct a.
+    + destruct fp1; try congruence.
+      eauto.
+    + destruct fp1; try congruence.
+      destruct (find_fields fid fpl) eqn: FIND; try congruence.
+      repeat destruct p. eauto.
+    + destruct fp1; try congruence.
+      destruct ty; try congruence.
+      destruct ident_eq; try congruence.
+      destruct list_eq_dec; try congruence.
+      destruct ident_eq; try congruence.
+      eauto.
+Qed.
+
+Lemma get_footprint_app_inv: forall phl1 phl2 fp1 fp2,
+    get_footprint (phl1 ++ phl2) fp1 = Some fp2 ->
+    exists fp3,
+      get_footprint phl1 fp1 = Some fp3
+      /\ get_footprint phl2 fp3 = Some fp2.
+Proof.
+  induction phl1; simpl; intros; eauto.
+  destruct a.
+  - destruct fp1; try congruence.
+    eauto.
+  - destruct fp1; try congruence.
+    destruct (find_fields fid fpl) eqn: FIND; try congruence.
+    repeat destruct p. eauto.
+  - destr_fp_enum fp1 ty.
+    eauto.
+Qed.
+    
+Lemma get_loc_footprint_eq: forall l fp b ofs b1 ofs1 fp1,
+    get_loc_footprint l fp b ofs = Some (b1, ofs1, fp1) ->
+    get_footprint l fp = Some fp1.
+Proof.
+  induction l; intros.
+  - simpl in H. inv H. auto.
+  - simpl in *. destruct a.
+    + destruct fp; try congruence.
+      eauto.
+    + destruct fp; try congruence.
+      destruct (find_fields fid fpl) eqn: FIND; try congruence.
+      repeat destruct p. eauto.
+    + destruct fp; try congruence.
+      destruct ty; try congruence.
+      destruct ident_eq; try congruence.
+      destruct list_eq_dec; try congruence.
+      destruct ident_eq; try congruence.
+      eauto.
+Qed.
+
+Lemma get_set_disjoint_paths_aux: forall phl1 phl2 fp1 fp2 fp b ofs,
+    paths_disjoint phl1 phl2 ->
+    set_footprint phl1 fp fp1 = Some fp2 ->
+    get_loc_footprint phl2 fp1 b ofs = get_loc_footprint phl2 fp2 b ofs.
+Proof.
+  induction phl1; intros.
+  - inv H.
+  - inv H.
+    + simpl in *.
+      destruct a.
+      * destruct fp1; try congruence.
+        destruct (set_footprint phl1 fp fp1) eqn: A; try congruence.
+        inv H0.
+        destruct p2; try congruence; auto.
+      * destruct fp1; try congruence.
+        destruct (find_fields fid fpl) eqn: FIND; try congruence.
+        repeat destruct p. 
+        destruct (set_footprint phl1 fp f) eqn: A; try congruence.
+        inv H0.
+        destruct p2; try congruence; auto.
+        destruct (ident_eq fid fid0); try congruence.
+        exploit find_fields_some; eauto. intros (B1 & B2). subst.
+        destruct (find_fields fid0 fpl) eqn: FIND1.
+        -- repeat destruct p.
+           exploit find_fields_some; eauto. intros (B3 & B4). subst.           
+           erewrite find_fields_set_spec; eauto.
+           destruct peq; try congruence.
+        -- destruct (find_fields fid0 (set_field i f0 fpl)) eqn: F1; try congruence.
+           repeat destruct p.
+           exploit find_fields_some; eauto. intros (B3 & B4). subst.
+           exploit find_fields_different_field; eauto. congruence.
+      * destr_fp_enum fp1 ty.
+        destruct (set_footprint phl1 fp fp1) eqn: A; try congruence.
+        inv H0.
+        destruct p2; try congruence.
+        destruct (type_eq (Tvariant orgs id) ty); try congruence.
+        -- subst.
+           destruct (ident_eq fid0 fid); try congruence.
+           destruct ident_eq; try congruence.
+           destruct list_eq_dec; try congruence.
+           destruct ident_eq; try congruence.
+        -- destruct ty; try congruence.
+           destruct ident_eq; try congruence.
+           destruct list_eq_dec; try congruence.
+    + simpl in *. destruct a.
+      * destruct fp1; try congruence.
+        destruct (set_footprint phl1 fp fp1) eqn: A; try congruence.
+        inv H0. eauto.
+      * destruct fp1; try congruence.
+        destruct (find_fields fid fpl) eqn: FIND; try congruence.
+        repeat destruct p. 
+        destruct (set_footprint phl1 fp f) eqn: A; try congruence.
+        inv H0.
+        exploit find_fields_some; eauto. intros (B1 & B2). subst.
+        erewrite find_fields_set_spec; eauto.
+        destruct peq; try congruence. eauto.
+      * destr_fp_enum fp1 ty.
+        destruct (set_footprint phl1 fp fp1) eqn: A; try congruence.
+        inv H0.
+        destruct ident_eq; try congruence.
+        destruct list_eq_dec; try congruence.
+        destruct ident_eq; try congruence. eauto.
+Qed.           
+        
+Lemma get_set_disjoint_paths : forall phl1 phl2 id e fpm1 fpm2 fp,
+    paths_disjoint phl1 phl2 ->
+    set_footprint_map (id, phl1) fp fpm1 = Some fpm2 ->
+    get_loc_footprint_map e (id, phl2) fpm1 = get_loc_footprint_map e (id, phl2) fpm2.
+Proof.
+  intros. simpl in *.
+  destruct (e!id) eqn: A; auto. destruct p.
+  destruct (fpm1 ! id) eqn: B; try congruence.
+  destruct (set_footprint phl1 fp f) eqn: C; try congruence.
+  inv H0. rewrite PTree.gss.
+  eapply get_set_disjoint_paths_aux; eauto.
+Qed.
+
+Lemma get_set_different_local : forall phl1 phl2 id1 id2 e fpm1 fpm2 fp,
+    id1 <> id2 ->
+    set_footprint_map (id1, phl1) fp fpm1 = Some fpm2 ->
+    get_loc_footprint_map e (id2, phl2) fpm1 = get_loc_footprint_map e (id2, phl2) fpm2.
+Proof.
+  intros. simpl in *.
+  destruct (e! id2) eqn: A; auto. destruct p.
+  destruct (fpm1 ! id1) eqn: B; try congruence.
+  destruct (set_footprint phl1 fp f) eqn: C; try congruence. inv H0.
+  rewrite PTree.gso; eauto.
+Qed.
+
+(* The footprints of two different subfields are disjoint *)
+Lemma footprint_norepet_fields_disjoint: forall (fpl: list (ident * Z * footprint)) id1 id2 fofs1 fofs2 fp1 fp2,
+    list_norepet (flat_map (fun '(_, _, fp) => footprint_flat fp) fpl) ->
+    In (id1, fofs1, fp1) fpl ->
+    In (id2, fofs2, fp2) fpl ->
+    id1 <> id2 ->
+    list_disjoint (footprint_flat fp1) (footprint_flat fp2).
+Proof.
+  induction fpl; simpl; intros; try contradiction.
+  destruct a. destruct p. 
+  eapply list_norepet_app in H. destruct H as (A1 & A2 & A3).
+  destruct H0; destruct H1.
+  - inv H. inv H0. congruence.
+  - inv H. red. intros. intro.
+    eapply A3. eauto.
+    eapply in_flat_map. exists (id2, fofs2, fp2). eauto. auto.
+  - inv H0. red. intros. intro.
+    eapply A3. eauto.
+    eapply in_flat_map. exists (id1, fofs1, fp1). eauto. auto.
+  - eauto.
+Qed.
+
+Lemma app_norepet_inv_tail: forall (l1 l2 l3 l4: list (positive * (block * type))) (id1: ident) (b: block) (ty1: type) id2 ty2,
+    l1 ++ (id1, (b, ty1)) :: l2 = l3 ++ (id2, (b, ty2)) :: l4 ->
+    ~ In b (map (fun elt : positive * (block * type) => fst (snd elt)) l1) ->
+    ~ In b (map (fun elt : positive * (block * type) => fst (snd elt)) l2) ->
+    ~ In b (map (fun elt : positive * (block * type) => fst (snd elt)) l3) ->
+    ~ In b (map (fun elt : positive * (block * type) => fst (snd elt)) l4) ->
+    id1 = id2.
+Proof.
+  induction l1; simpl; intros; auto.
+  - destruct l3; simpl in *.
+    + inv H. auto.
+    + destruct p. destruct p0.
+      inv H. simpl in *. eapply Decidable.not_or in H2.
+      destruct H2. congruence.
+  - destruct a. destruct p0.
+    destruct l3; simpl in *.
+    + inv H. eapply Decidable.not_or in H0.
+      destruct H0. congruence.
+    + inv H. simpl in *.
+      eapply IHl1; eauto.
+Qed.
+
+      
+Lemma footprint_norepet_env_disjoint: forall e id1 id2 b1 b2 ty1 ty2,
+    list_norepet (footprint_of_env e) ->
+    e ! id1 = Some (b1, ty1) ->
+    e ! id2 = Some (b2, ty2) ->
+    id1 <> id2 ->
+    b1 <> b2.
+Proof.
+  intros until ty2. intros NOREP E1 E2 NEQ.
+  intro. eapply NEQ. subst.
+  unfold footprint_of_env in NOREP.
+  generalize NOREP as NOREP1. intros.
+  exploit PTree.elements_remove. eapply E1. intros (l1 & l2 & A1 & A2).  
+  rewrite A1 in NOREP. rewrite map_app in NOREP. simpl in NOREP.
+  exploit PTree.elements_remove. eapply E2. intros (l3 & l4 & A3 & A4).
+  rewrite A3 in NOREP1. rewrite map_app in NOREP1. simpl in NOREP1.
+  rewrite A1 in A3.
+  eapply list_norepet_app in NOREP as (N1 & N2 & N3). inv N2.
+  eapply list_norepet_app in NOREP1 as (N4 & N5 & N6). inv N5.  
+  eapply app_norepet_inv_tail; eauto.
+  intro. eapply N3; eauto. simpl. auto.
+  intro. eapply N6; eauto. simpl. auto.
+Qed.
+
+  
+Lemma footprint_norepet_fields_norepet: forall (fpl: list (ident * Z * footprint)) id fofs fp,
+    list_norepet (flat_map (fun '(_, _, fp) => footprint_flat fp) fpl) ->
+    In (id, fofs, fp) fpl ->
+    list_norepet (footprint_flat fp).
+Proof.
+  induction fpl; simpl; intros; try contradiction.
+  destruct a. destruct p. destruct H0.
+  - inv H0. eapply list_norepet_app in H. destruct H as (A1 & A2 & A3).
+    auto.
+  - eapply list_norepet_app in H. destruct H as (A1 & A2 & A3).
+    eauto.
+Qed.
+
+
+(* This lemma indicates that the footprint is a non-cyclic tree. *)
+Lemma get_footprint_norepet: forall phl fp fp1,
+    list_norepet (footprint_flat fp) ->
+    get_footprint phl fp = Some fp1 ->
+    list_norepet (footprint_flat fp1).
+Proof.
+  induction phl; intros until fp1; intros NOREP1 GFP; simpl in *.
+  - inv GFP. auto.
+  - destruct a.
+    + destruct fp; try congruence.
+      simpl in *. inv NOREP1.
+      eapply IHphl; eauto.
+    + destruct fp; try congruence.
+      destruct (find_fields fid fpl) eqn: FIND; try congruence.
+      repeat destruct p.
+      exploit find_fields_some; eauto. intros (A1 & A2). subst.
+      eapply IHphl. 2: eapply GFP.
+      eapply footprint_norepet_fields_norepet; eauto.
+    + destr_fp_enum fp ty.
+      simpl in *. eauto.
+Qed.
+
+
+(* This lemma indicates that the footprint is a non-cyclic tree. *)
+Lemma get_loc_footprint_norepet: forall phl fp b ofs b1 ofs1 fp1,
+    list_norepet (footprint_flat fp) ->
+    get_loc_footprint phl fp b ofs = Some (b1, ofs1, fp1) ->
+    ~ In b (footprint_flat fp) ->
+    list_norepet (footprint_flat fp1)
+    /\ ~ In b1 (footprint_flat fp1).
+Proof.
+  induction phl; intros until fp1; intros NOREP1 GFP NIN; simpl in *.
+  - inv GFP. auto.
+  - destruct a.
+    + destruct fp; try congruence.
+      simpl in *. inv NOREP1.
+      eapply IHphl; eauto.
+    + destruct fp; try congruence.
+      destruct (find_fields fid fpl) eqn: FIND; try congruence.
+      repeat destruct p.
+      exploit find_fields_some; eauto. intros (A1 & A2). subst.
+      eapply IHphl. 2: eapply GFP.
+      eapply footprint_norepet_fields_norepet; eauto.
+      intro. eapply NIN. simpl.
+      eapply in_flat_map; eauto.
+    + destr_fp_enum fp ty.
+      simpl in *. eauto.
+Qed.
+
+Lemma norepet_flat_fp_map_element: forall fpm id fp,
+    fpm ! id = Some fp ->
+    list_norepet (flat_fp_map fpm) ->
+    list_norepet (footprint_flat fp).
+Proof.
+  intros. eapply PTree.elements_remove in H.
+  destruct H as (l1 & L2 & A & B).
+  unfold flat_fp_map in H0.
+  rewrite A in H0.
+  erewrite flat_map_app in H0. 
+  eapply list_norepet_app in H0. destruct H0 as (C & D & E).
+  simpl in D. eapply list_norepet_app in D. destruct D.
+  auto.
+Qed.
+
+Lemma norepet_flat_fp_map_element_disjoint: forall fpm id1 id2 fp1 fp2,
+    fpm ! id1 = Some fp1 ->
+    fpm ! id2 = Some fp2 ->
+    id1 <> id2 ->
+    list_norepet (flat_fp_map fpm) ->
+    list_disjoint (footprint_flat fp1) (footprint_flat fp2).
+Proof.
+  intros. unfold flat_fp_map in H2.
+  eapply PTree.elements_correct in H.
+  eapply PTree.elements_correct in H0.
+  generalize dependent (PTree.elements fpm).
+  induction l; intros; simpl in *; try contradiction.
+  destruct a. destruct H.
+  - inv H. destruct H0. inv H. try congruence.
+    eapply list_norepet_app in H2 as (N1 & N2 & N3).
+    simpl in *. red. intros.
+    eapply N3; auto.
+    eapply in_flat_map; eauto.
+  - destruct H0. inv H0.
+    + eapply list_norepet_app in H2 as (N1 & N2 & N3).
+      simpl in *. eapply list_disjoint_sym. red. intros.
+      eapply N3; auto.
+      eapply in_flat_map; eauto.
+    + eapply list_norepet_app in H2 as (N1 & N2 & N3).
+      eauto.
+Qed.
+
+    
+(** separating a footprint from the well-formed
+footprint map *)
+Lemma get_loc_footprint_map_norepet: forall phl id fpm b1 ofs1 fp1 e,
+    list_norepet (flat_fp_map fpm) ->
+    get_loc_footprint_map e (id, phl) fpm = Some (b1, ofs1, fp1) ->
+    (* we require that the stack blocks and the blocks in fpm are disjoint *)
+    list_disjoint (footprint_of_env e) (flat_fp_map fpm) ->
+    list_norepet (footprint_flat fp1)
+    /\ ~ In b1 (footprint_flat fp1).
+Proof.
+  intros until e. intros NOREP1 GFP DIS.
+  unfold get_loc_footprint_map in GFP.
+  destruct (e!id) eqn: A; try congruence.
+  destruct p.
+  destruct (fpm!id) eqn: B; try congruence.
+  eapply get_loc_footprint_norepet; eauto.
+  eapply norepet_flat_fp_map_element; eauto.
+  intro. eapply DIS. eapply in_footprint_of_env; eauto.
+  eapply in_footprint_flat_fp_map; eauto. auto.
+Qed.  
+
+Lemma set_footprint_incl: forall phl fp1 fp2 fp b,
+    set_footprint phl fp fp1 = Some fp2 ->
+    In b (footprint_flat fp2) ->
+    In b (footprint_flat fp1)
+    \/ In b (footprint_flat fp).
+Proof.
+  induction phl; simpl; intros.
+  - inv H. auto.
+  - destruct a.
+    + destruct fp1; try congruence. 
+      destruct (set_footprint phl fp fp1) eqn: A; try congruence.
+      inv H. simpl in *. destruct H0; eauto.
+      exploit IHphl; eauto. intros [E1|E2]; eauto.
+    + destruct fp1; try congruence.
+      destruct (find_fields fid fpl) eqn: FIND; try congruence.
+      repeat destruct p.
+      exploit find_fields_some; eauto. intros (A1 & A2). subst.
+      destruct (set_footprint phl fp f) eqn: A; try congruence.
+      inv H. simpl in *.
+      exploit find_fields_split; eauto.
+      intros (l1 & l2 & B1 & B2). subst.
+      erewrite set_fields_split in H0; eauto. rewrite flat_map_app in *.
+      simpl in *.      
+      rewrite !in_app in H0.
+      rewrite !in_app. destruct H0; auto.
+      destruct H; auto.
+      exploit IHphl; eauto. intros [E1|E2]; eauto.
+    + destr_fp_enum fp1 ty.
+      destruct (set_footprint phl fp fp1) eqn: A; try congruence.
+      inv H. simpl in *. eauto.
+Qed.
+      
+Lemma set_footprint_norepet: forall phl fp1 fp2 vfp,
+    set_footprint phl vfp fp1 = Some fp2 ->
+    list_norepet (footprint_flat fp1) ->
+    list_norepet (footprint_flat vfp) ->
+    list_disjoint (footprint_flat fp1) (footprint_flat vfp) ->
+    list_norepet (footprint_flat fp2).
+Proof.
+  induction phl; intros until vfp; intros SET N1 N2 DIS; simpl in *.
+  - inv SET. auto.
+  - destruct a.
+    + destruct fp1; try congruence. 
+      destruct (set_footprint phl vfp fp1) eqn: A; try congruence.
+      inv SET. simpl in *.       
+      inv N1. econstructor; eauto.
+      intro. exploit set_footprint_incl; eauto.
+      intros [E1|E2]; try congruence.
+      eapply DIS; eauto. simpl. auto.
+      eapply IHphl; eauto.
+      eapply list_disjoint_cons_left; eauto.
+    + destruct fp1; try congruence.
+      destruct (find_fields fid fpl) eqn: FIND; try congruence.
+      repeat destruct p.
+      exploit find_fields_some; eauto. intros (A1 & A2). subst.
+      destruct (set_footprint phl vfp f) eqn: A; try congruence.
+      inv SET. simpl in *.
+      exploit IHphl; eauto.
+      eapply footprint_norepet_fields_norepet; eauto.
+      red. intros. eapply DIS; eauto.
+      eapply in_flat_map; eauto.
+      intros NF.
+      exploit find_fields_split; eauto.
+      intros (l1 & l2 & B1 & B2). subst.
+      erewrite set_fields_split; eauto. rewrite flat_map_app in *.
+      simpl in *.
+      eapply list_norepet_append_commut2.
+      eapply list_norepet_append_commut2 in N1.
+      rewrite app_assoc in *. eapply list_norepet_app.
+      eapply list_norepet_app in N1 as (N3 & N4 & N5).
+      repeat apply conj; auto.
+      red. intros.
+      exploit set_footprint_incl; eauto. intros [E1|E2].
+      eapply N5; eauto.
+      eapply DIS; eauto.
+      rewrite in_app in H.
+      rewrite !in_app. destruct H; auto.
+    + destr_fp_enum fp1 ty.
+      destruct (set_footprint phl vfp fp1) eqn: A; try congruence.
+      inv SET. simpl in *. eauto.
+Qed.
+
+      
+(* Key lemma to simplify the proof of set_disjoint_footprint_norepet *)
+Lemma PTree_remove_elements_eq {A: Type}: forall id (v: A) m,
+    PTree.elements (PTree.remove id m) = PTree.elements (PTree.remove id (PTree.set id v m)).
+Proof.
+  intros.
+  eapply PTree.elements_extensional.
+  intros. rewrite !PTree.grspec.
+  destruct PTree.elt_eq; subst; auto.
+  rewrite PTree.gso; eauto.
+Qed.
+
+(* norepet (l ++ fpm) where l is a general list which can
+    represent other elements in the frame *)
+Lemma set_disjoint_footprint_norepet: forall fpm1 fpm2 vfp id phl,
+    list_norepet (footprint_flat vfp) ->
+    list_norepet (flat_fp_map fpm1) ->
+    set_footprint_map (id, phl) vfp fpm1 = Some fpm2 ->
+    list_disjoint (flat_fp_map fpm1) (footprint_flat vfp) ->
+    list_norepet (flat_fp_map fpm2).
+Proof.
+  intros until phl. intros NVFP NOREP SET DIS. simpl in *.
+  destruct (fpm1 ! id) eqn: A; try congruence.
+  destruct (set_footprint phl vfp f) eqn: B; try congruence. inv SET.
+  (* show that f0 is norepet *)
+  exploit norepet_flat_fp_map_element; eauto. intros NF.
+  exploit set_footprint_norepet; eauto.
+  red. intros. eapply DIS. eapply in_footprint_flat_fp_map; eauto. auto.
+  intros NF0.
+  unfold flat_fp_map in *.
+  exploit PTree.elements_remove. eauto. intros (l1 & l2 & A1 & A2).
+  exploit PTree.elements_remove. instantiate (3 := (PTree.set id f0 fpm1)).
+  eapply PTree.gss; eauto. intros (l3 & l4 & A3 & A4).
+  erewrite <- PTree_remove_elements_eq in A4. rewrite A2 in A4.
+  rewrite A1 in *. rewrite A3 in *.  
+  rewrite !flat_map_app in *. simpl in *.
+  eapply list_norepet_append_commut2.
+  eapply list_norepet_append_commut2 in NOREP.
+  rewrite app_assoc in *. 
+  rewrite <- flat_map_app in *. rewrite <- A4.
+  eapply list_norepet_app in NOREP as (N1 & N2 & N3).
+  eapply list_norepet_app. split. auto.
+  split.
+  (* f0 is norepet *)
+  auto.
+  (* disjointness *)
+  red. intros.
+  exploit set_footprint_incl; eauto.
+  intros [E1|E2].
+  (* x in l1 ++l2 and y in f *)
+  eapply N3. auto. auto.
+  (* x in l1 ++l2 and y in vfp *)
+  eapply DIS.
+  rewrite flat_map_app in H. eapply in_app in H.
+  rewrite !in_app. destruct H; auto. auto.
+Qed.
+
+Lemma empty_footprint_flat: forall fp,
+    footprint_flat (clear_footprint_rec fp) = nil.
+Proof.
+  induction fp using strong_footprint_ind; simpl; auto.
+  induction fpl; simpl; auto.
+  destruct a. destruct p. erewrite H. simpl.
+  eapply IHfpl. intros. eapply H. eapply in_cons; eauto.
+  econstructor. eauto.
+Qed.
+
+Lemma empty_footprint_disjoint: forall fp1 fp2,
+    list_disjoint fp1 (footprint_flat (clear_footprint_rec fp2)).
+Proof.
+  intros. rewrite empty_footprint_flat. red. intros. inv H0.
+Qed.
+
+Lemma get_footprint_incl: forall phl fp fp1,
+    get_footprint phl fp = Some fp1 ->
+    incl (footprint_flat fp1) (footprint_flat fp).
+Proof.
+  induction phl; intros; simpl in *.
+  - inv H. eapply incl_refl.
+  - destruct a.
+    + destruct fp; try congruence.
+      simpl. red.
+      intros. eapply in_cons. eapply IHphl; eauto.
+    + destruct fp; try congruence.
+      destruct (find_fields fid fpl) eqn: FIND; try congruence.
+      repeat destruct p.
+      simpl. red. intros. eapply in_flat_map.
+      eapply IHphl in H0; eauto.
+      eapply find_fields_some in FIND. destruct FIND. subst.
+      exists (i, z, f). auto.
+    + destruct fp; try congruence.
+      destruct ty; try congruence.
+      destruct ident_eq; subst; try congruence.
+      destruct list_eq_dec; subst; try congruence.
+      destruct ident_eq; subst; try congruence.
+      simpl. eauto.
+Qed.
+
+
+(* The footprint is included in the source footprint *)
+Lemma get_loc_footprint_incl: forall phl fp b ofs b1 ofs1 fp1,
+    get_loc_footprint phl fp b ofs = Some (b1, ofs1, fp1) ->
+    incl (footprint_flat fp1) (footprint_flat fp).
+Proof.
+  intros. eapply get_footprint_incl.
+  eapply get_loc_footprint_eq. eauto.
+Qed.  
+
+Lemma get_loc_footprint_map_incl: forall phl fpm b1 ofs1 fp1 le id,
+    get_loc_footprint_map le (id, phl) fpm = Some (b1, ofs1, fp1) ->
+    incl (footprint_flat fp1) (flat_fp_map fpm).
+Proof.
+  intros. simpl in H. destruct (le!id) in H; try congruence.
+  destruct p. destruct (fpm!id) eqn: FPM; try congruence.
+  red. intros. eapply get_loc_footprint_incl in H0; eauto.
+  unfold flat_fp_map.
+  eapply in_flat_map; eauto.
+  exists (id, f). simpl. split; auto.
+  eapply PTree.elements_correct. auto.
+Qed.
+
+
+Lemma get_loc_footprint_in: forall phl fp1 b1 ofs1 b2 ofs2 fp2,
+    get_loc_footprint phl fp1 b1 ofs1 = Some (b2, ofs2, fp2) ->
+    In b2 (b1 :: footprint_flat fp1).
+Proof.
+  induction phl; intros.
+  - simpl in H. inv H. econstructor; auto.
+  - simpl in H. destruct a.
+    + destruct fp1; try congruence.
+      exploit IHphl; eauto. intros IN. inv IN.
+      eapply in_cons. simpl. auto.
+      eapply in_cons. simpl. auto.
+    + destruct fp1; try congruence.
+      destruct (find_fields fid fpl) eqn: FIND; try congruence.
+      repeat destruct p.
+      exploit find_fields_some; eauto. intros (A1 & A2). subst.
+      exploit IHphl; eauto. intros IN. inv IN.
+      econstructor. auto.
+      eapply in_cons. simpl. eapply in_flat_map; eauto.
+    + destr_fp_enum fp1 ty.
+      exploit IHphl; eauto.
+Qed.
+
+(* The block obtained from get_loc_footprint_map comes from
+   stack or the footprint map *)
+Lemma get_loc_footprint_map_in_range: forall phl id fpm le b ofs fp,
+    get_loc_footprint_map le (id, phl) fpm = Some (b, ofs, fp) ->
+    In b (footprint_of_env le ++ flat_fp_map fpm).
+Proof.
+  intros. simpl in *.
+  destruct (le!id) eqn: A; try congruence.
+  destruct p.
+  destruct (fpm!id) eqn: B; try congruence.
+  exploit get_loc_footprint_in; eauto.
+  intros IN. inv IN.
+  eapply in_app_iff. left. eapply in_footprint_of_env; eauto.
+  eapply in_app_iff. right. eapply in_footprint_flat_fp_map; eauto.
+Qed.
+
+Lemma in_app_commut {A: Type} : forall (l1 l2 l3: list A) a,
+      In a (l1 ++ l2 ++ l3) <-> In a (l1 ++ l3 ++ l2).
+Proof.
+  intros. split; intros.
+  - rewrite !in_app in *.
+    repeat destruct H; auto.
+  - rewrite !in_app in *.
+    repeat destruct H; auto.
+Qed.
+
+Lemma set_footprint_map_incl: forall fpm1 fpm2 fp id phl b,
+    set_footprint_map (id, phl) fp fpm1 = Some fpm2 ->
+    In b (flat_fp_map fpm2) ->
+    In b (flat_fp_map fpm1) \/ In b (footprint_flat fp).
+Proof.
+  intros.
+  simpl in *. destruct (fpm1!id) eqn: A; try congruence.
+  destruct (set_footprint phl fp f) eqn: B; try congruence.
+  inv H. 
+  unfold flat_fp_map in *.
+  exploit PTree.elements_remove. eauto. intros (l1 & l2 & A1 & A2).
+  exploit PTree.elements_remove. instantiate (3 := (PTree.set id f0 fpm1)).
+  eapply PTree.gss; eauto. intros (l3 & l4 & A3 & A4).
+  erewrite <- PTree_remove_elements_eq in A4. rewrite A2 in A4.
+  rewrite A1 in *. rewrite A3 in *.  
+  rewrite flat_map_app in *. simpl in *.
+  erewrite in_app_commut in *. rewrite app_assoc in *.
+  rewrite <- flat_map_app in *. rewrite A4 in *.
+  rewrite in_app in *. destruct H0; auto.
+  exploit set_footprint_incl; eauto. intros [E1|E2]; auto.
+Qed.
+  
+Lemma get_set_disjoint_footprint: forall phl fp fp' fp1 fp2,
+    get_footprint phl fp = Some fp1 ->
+    set_footprint phl fp2 fp = Some fp' ->
+    list_disjoint (footprint_flat fp1) (footprint_flat fp2) ->
+    list_norepet (footprint_flat fp) ->
+    list_disjoint (footprint_flat fp') (footprint_flat fp1).
+Proof.
+  induction phl; intros until fp2; intros GFP SFP DIS NOREP; simpl in *.
+  - inv GFP. inv SFP.
+    eapply list_disjoint_sym. auto.
+  - destruct a.
+    + destruct fp; try congruence.
+      destruct (set_footprint phl fp2 fp) eqn: S1; try congruence.
+      inv SFP. simpl in *.
+      red. intros. inv H.
+      * inv NOREP. intro. subst. eapply H2.
+        eapply get_footprint_incl; eauto.
+      * eapply IHphl; eauto.
+        inv NOREP; auto.
+    + destruct fp; try congruence.
+      destruct (find_fields fid fpl) eqn: FIND; try congruence.
+      repeat destruct p.
+      exploit find_fields_some. eapply FIND. intros (A1 & A2). subst.
+      destruct (set_footprint phl fp2 f) eqn: S1; try congruence.
+      inv SFP. simpl in *.
+      exploit find_fields_split; eauto.
+      intros (l1 & l2 & B1 & B2). subst.
+      erewrite set_fields_split; eauto.
+      erewrite flat_map_app in NOREP.
+      eapply list_norepet_app in NOREP as (N1 & N2 & N3).
+      red. intros.
+      rewrite flat_map_app in H.
+      eapply in_app_iff in H. destruct H.
+      * eapply N3. eauto.
+        simpl. eapply in_app. left.
+        eapply get_footprint_incl; eauto.
+      * simpl in H. eapply in_app in H.
+        destruct H.
+        (* adhoc *)
+        -- eapply IHphl; eauto.
+           simpl in N2. eapply list_norepet_append_left. eauto.
+        -- simpl in N2.
+           eapply list_norepet_app in N2 as (N4 & N5 & N6).
+           intro. subst. eapply N6; eauto.
+           eapply get_footprint_incl; eauto.
+    + destr_fp_enum fp ty.
+      destruct (set_footprint phl fp2 fp) eqn: S1; try congruence.
+      inv SFP. simpl in *. eapply IHphl; eauto.
+Qed.
+
+(* Set a footprint also remove the original one out. This removed
+   footprint is disjoint with the updated footprint map *)
+Lemma get_set_disjoint_footprint_map: forall l i fpm1 fpm2 b ofs fp1 fp2 le,
+    get_loc_footprint_map le (i, l) fpm1 = Some (b, ofs, fp1) ->
+    set_footprint_map (i, l) fp2 fpm1 = Some fpm2 ->
+    list_disjoint (footprint_flat fp1) (footprint_flat fp2) ->
+    list_norepet (flat_fp_map fpm1) ->
+    list_disjoint (flat_fp_map fpm2) (footprint_flat fp1).
+Proof.
+  intros. simpl in *.
+  destruct (le ! i) eqn: A1; try congruence. destruct p.
+  destruct (fpm1 ! i) eqn: A2; try congruence.
+  destruct (set_footprint l fp2 f) eqn: A3; try congruence. inv H0.
+  red. intros.
+  eapply in_flat_map in H0.
+  destruct H0 as ((id & fp) & IN1 & IN2). 
+  eapply PTree.elements_complete in IN1. rewrite PTree.gsspec in IN1.
+  destruct peq in IN1.
+  - inv IN1.
+    eapply get_set_disjoint_footprint; eauto.
+    eapply get_loc_footprint_eq; eauto.
+    eapply norepet_flat_fp_map_element; eauto.
+  - eapply norepet_flat_fp_map_element_disjoint. eapply IN1. eapply A2.
+    auto. auto. auto.
+    eapply get_loc_footprint_incl; eauto.
+Qed.      
+    
+Lemma get_clear_footprint_incl1: forall phl fp1 fp2 fp3,
+    get_footprint phl fp1 = Some fp2 ->
+    set_footprint phl (clear_footprint_rec fp2) fp1 = Some fp3 ->
+    incl (footprint_flat fp2 ++ footprint_flat fp3) (footprint_flat fp1).
+Proof.
+  intros. red. intros.
+ eapply in_app_iff in H1. destruct H1.
+ eapply get_footprint_incl; eauto.
+ exploit set_footprint_incl; eauto.
+ intros [A|B]; auto.
+ rewrite empty_footprint_flat in B. inv B.
+Qed.
+
+
+Lemma get_clear_footprint_incl2: forall phl fp1 fp2 fp3,
+    get_footprint phl fp1 = Some fp2 ->
+    set_footprint phl (clear_footprint_rec fp2) fp1 = Some fp3 ->
+    incl (footprint_flat fp1) (footprint_flat fp2 ++ footprint_flat fp3).
+Proof.
+  induction phl; simpl in *; intros.
+  - inv H0. inv H. rewrite empty_footprint_flat. rewrite app_nil_r.
+    eapply incl_refl.
+  - destruct a.
+    + destruct fp1; try congruence.
+      destruct (set_footprint phl (clear_footprint_rec fp2) fp1) eqn: A; try congruence.
+      inv H0. 
+      generalize (IHphl fp1 fp2 f H A). intros INCL1.
+      red. simpl. intros. destruct H0; subst.
+      * eapply in_app_iff. right. econstructor. auto.
+      * eapply INCL1 in H0. eapply in_app_iff in H0. destruct H0.
+        eapply in_app_iff; eauto.
+        eapply in_app_iff. right. eapply in_cons; auto.
+    + destruct fp1; try congruence.
+      destruct (find_fields fid fpl) eqn: FIND; try congruence.
+      repeat destruct p.
+      destruct (set_footprint phl (clear_footprint_rec fp2) f) eqn: A; try congruence.
+      inv H0. 
+      exploit find_fields_some; eauto. intros (B1 & B2). subst.
+      generalize (IHphl f fp2 f0 H A). intros INCL1.
+      red. simpl. intros.
+      eapply in_flat_map in H0. destruct H0 as (((fid & fofs) & ffp) & IN1 & IN2).
+      exploit find_fields_split; eauto. intros (l1 & l2 & A1 & A2). subst.
+      erewrite set_fields_split; eauto.
+      rewrite flat_map_app. simpl. rewrite !in_app. rewrite !in_app in IN1.
+      destruct IN1.
+      * right. left. eapply in_flat_map; eauto.
+      * inv H0.
+        -- inv H1. eapply INCL1 in IN2.
+           eapply in_app in IN2. destruct IN2; auto.
+        -- repeat right. eapply in_flat_map; eauto.
+    + destr_fp_enum fp1 ty.
+      destruct (set_footprint phl (clear_footprint_rec fp2) fp1) eqn: A; try congruence.
+      inv H0. simpl. eauto.
+Qed.
+
+Lemma get_clear_footprint_equiv: forall phl fp1 fp2 fp3,
+    get_footprint phl fp1 = Some fp2 ->
+    set_footprint phl (clear_footprint_rec fp2) fp1 = Some fp3 ->
+    list_equiv (footprint_flat fp2 ++ footprint_flat fp3) (footprint_flat fp1).
+Proof.
+  intros. split.
+  eapply get_clear_footprint_incl1; eauto.
+  eapply get_clear_footprint_incl2; eauto.
+Qed.
+
+
+(* (fpm\fp ) * fp = fpm: this lemma relies on wf_env so we put here *)
+Lemma get_clear_footprint_map_equiv: forall fpm1 fpm2 fp le id phl b ofs,
+    get_loc_footprint_map le (id, phl) fpm1 = Some (b, ofs, fp) ->
+    clear_footprint_map le (id, phl) fpm1 = Some fpm2 ->
+    list_equiv (footprint_flat fp ++ flat_fp_map fpm2) (flat_fp_map fpm1).
+Proof.
+  intros until ofs. intros GFP CLR.
+  unfold clear_footprint_map in CLR. rewrite GFP in CLR.
+  split.   
+  - intros. eapply in_app_iff in H. destruct H.
+    + eapply get_loc_footprint_map_incl; eauto.
+    + exploit set_footprint_map_incl; eauto.
+      rewrite empty_footprint_flat. simpl. intros [A|B]; try inv B; auto.
+  - intros IN.
+    simpl in *. destruct (le ! id) eqn: A1; try congruence.
+    destruct p.
+    destruct (fpm1 ! id) eqn: A2; try congruence.
+    destruct (set_footprint phl (clear_footprint_rec fp) f) eqn: A3; try congruence.
+    inv CLR.
+    generalize GFP as GFP1. intros. eapply get_loc_footprint_eq in GFP1.
+    generalize (get_clear_footprint_equiv _ _ _ _ GFP1 A3). intros EQV.
+    eapply in_flat_map in IN as ((id1 & fp2) & IN3 & IN4).
+    simpl in *. eapply PTree.elements_complete in IN3.
+    destruct (ident_eq id id1).
+    + subst. rewrite A2 in IN3. inv IN3.
+      eapply EQV in IN4. eapply in_app_iff in IN4. destruct IN4.
+      * eapply in_app; auto.
+      * eapply in_app_iff.
+        right.
+        eapply in_flat_map; eauto.
+        exists (id1, f0). split; eauto.
+        eapply PTree.elements_correct. eapply PTree.gss.
+    + eapply in_app. right.
+      eapply in_flat_map; eauto.
+      exists (id1, fp2). split; eauto.
+      eapply PTree.elements_correct. erewrite PTree.gso; eauto.
+Qed.
+
+
+(** ** Typing of the footprint: used to make sure the footprint is well-formed *)
+
+
+Definition name_members (membs: members) : list ident :=
+  map name_member membs.
+
+Section COMP_ENV.
+
+Variable ce: composite_env.
+
+(* Definition of wt_footprint (well-typed footprint). Intuitively, it
+says that the footprint is an abstract form of the syntactic type
+ty. We need an intermediate composite_env to act as the recursive
+guard to simulate the move checking because we do not allow unbounded
+appearence of shallow struct. What if we allow recursive struct in the
+footprint but if can be rule out in move checking? *)
+Inductive wt_footprint : type -> footprint -> Prop :=
+| wt_fp_emp: forall ty
+    (* It means that the location with this type is not
+        initialized or this location is scalar type *)
+    (WF: forall orgs id, ty <> Tstruct orgs id),
+    wt_footprint ty fp_emp
+| wt_fp_scalar: forall ty
+    (WF: scalar_type ty = true),
+    wt_footprint ty (fp_scalar ty)
+| wt_fp_struct: forall orgs id fpl co
+    (CO: ce ! id = Some co)
+    (STRUCT: co_sv co = Struct)
+    (** TODO: combine WT1 and WT2 elegantly. WT1 is used in getting
+    the sub-field's footprint. WT2 is used in proving the properties
+    of sub-field's footprint *)
+    (WT1: forall fid fty,
+        field_type fid co.(co_members) = OK fty ->
+        (* For simplicity, use find_field instead of In predicate *)
+        exists ffp fofs,
+          find_fields fid fpl = Some (fid, fofs, ffp)
+          /\ field_offset ce fid co.(co_members) = OK fofs
+          (* bound condition *)
+          /\ wt_footprint fty ffp)
+    (WT2: forall fid fofs ffp,
+        find_fields fid fpl = Some (fid, fofs, ffp) ->
+        exists fty,
+          field_type fid co.(co_members) = OK fty
+          /\ field_offset ce fid co.(co_members) = OK fofs
+          /\ wt_footprint fty ffp)
+    (* make sure that the flattened footprint list has the same order
+    as that of the members *)
+    (FLAT: name_footprints fpl = name_members (co_members co)),
+    (* This norepet property is used to ensure that set_field onlys
+    update one footprint instead of overriding some footprint with the
+    same name *)
+    (* (NOREP: list_norepet (name_footprints fpl)), *)
+    wt_footprint (Tstruct orgs id) (fp_struct id fpl)
+| wt_fp_enum: forall orgs id tagz fid fty fofs fp co
+    (CO: ce ! id = Some co)
+    (ENUM: co_sv co = TaggedUnion)
+    (TAG: list_nth_z co.(co_members) tagz = Some (Member_plain fid fty))
+    (* avoid some norepet properties *)
+    (FTY: field_type fid co.(co_members) = OK fty)
+    (FOFS: variant_field_offset ce fid co.(co_members) = OK fofs)
+    (WT: wt_footprint fty fp),
+    wt_footprint (Tvariant orgs id) (fp_enum id orgs tagz fid fofs fp)
+| wt_fp_box: forall ty b fp
+    (* this is ensured by bm_box *)
+    (WT: wt_footprint ty fp),
+    (* It is used to make sure that dropping any location within a
+    block does not cause overflow *)
+    wt_footprint (Tbox ty) (fp_box b (sizeof ce ty) fp).
+
+End COMP_ENV.
+
+
+(* The definition of wt_path should be a function instead of a
+relation. *)
+Inductive wt_path ce (ty: type) : list path -> type -> Prop :=
+| wt_path_nil: wt_path ce ty nil ty
+| wt_path_deref: forall phl ty1 ty2
+    (WP1: wt_path ce ty phl ty1)
+    (WP2: type_deref ty1 = OK ty2),
+    wt_path ce ty (phl ++ [ph_deref]) ty2
+| wt_path_field: forall phl orgs id co ty1 fid
+    (WP1: wt_path ce ty phl (Tstruct orgs id))
+    (WP2: ce ! id = Some co)
+    (WP3: field_type fid (co_members co) = OK ty1)
+    (WP4: co_sv co = Struct),
+    wt_path ce ty (phl++[ph_field fid]) ty1
+| wt_path_downcast: forall phl orgs id co ty1 fid
+    (WP1: wt_path ce ty phl (Tvariant orgs id))
+    (WP2: ce ! id = Some co)
+    (WP3: field_type fid (co_members co) = OK ty1)
+    (WP4: co_sv co = TaggedUnion),
+    wt_path ce ty (phl++[ph_downcast (Tvariant orgs id) fid]) ty1
+.
+
+Lemma wt_path_nil_inv: forall ce ty1 ty2,
+    wt_path ce ty1 nil ty2 ->
+    ty1 = ty2.
+Proof.
+  intros. inv H. auto.
+  1-3: destruct phl; inv H1.
+Qed.
+
+Lemma wt_path_deref_inv: forall ce ty1 ty2 phl,
+    wt_path ce ty1 (phl ++ [ph_deref]) ty2 ->
+    exists ty1', wt_path ce ty1 phl ty1'
+            /\ type_deref ty1' = OK ty2.
+Proof.
+  intros. inv H.
+  destruct phl; inv H1.
+  eapply app_inj_tail in H1. destruct H1. subst. eauto.
+  eapply app_inj_tail in H1. destruct H1. congruence.
+  eapply app_inj_tail in H1. destruct H1. congruence.
+Qed.
+
+Lemma wt_path_field_inv: forall ce ty1 ty2 phl fid,
+    wt_path ce ty1 (phl ++ [ph_field fid]) ty2 ->
+    exists id orgs co,
+      wt_path ce ty1 phl (Tstruct orgs id)
+      /\ ce ! id = Some co
+      /\ field_type fid (co_members co) = OK ty2
+      /\ co_sv co = Struct.
+Proof.
+  intros. inv H.
+  destruct phl; inv H1.
+  eapply app_inj_tail in H1. destruct H1. congruence.
+  eapply app_inj_tail in H1. destruct H1. inv H0.
+  exists id, orgs, co. eauto.
+  eapply app_inj_tail in H1. destruct H1. congruence.
+Qed.
+
+Lemma wt_path_downcast_inv: forall ce ty1 ty2 phl fid ty,
+    wt_path ce ty1 (phl ++ [ph_downcast ty fid]) ty2 ->
+    exists id orgs co,
+      ty = Tvariant orgs id                    
+      /\ wt_path ce ty1 phl (Tvariant orgs id)
+      /\ ce ! id = Some co
+      /\ field_type fid (co_members co) = OK ty2
+      /\ co_sv co = TaggedUnion.
+Proof.
+  intros. inv H.
+  destruct phl; inv H1.
+  eapply app_inj_tail in H1. destruct H1. congruence.
+  eapply app_inj_tail in H1. destruct H1. congruence.
+  eapply app_inj_tail in H1. destruct H1. inv H0.
+  exists id, orgs, co. eauto.
+Qed.
+
+
+Lemma wt_path_det: forall phl ty1 ty2 ty3 ce,
+    wt_path ce ty1 phl ty2 ->
+    wt_path ce ty1 phl ty3 ->
+    ty2 = ty3.
+Proof.
+  intro phl. cut (exists n, length phl = n); eauto. intros (n & LEN).
+  generalize dependent phl.
+  induction n; intros.
+  - eapply length_zero_iff_nil in LEN. subst.
+    eapply wt_path_nil_inv in H0. subst.
+    eapply wt_path_nil_inv in H. subst. auto.
+  - eapply length_S_inv in LEN.
+    destruct LEN as (l' & a & A & LEN). subst.
+    destruct a.
+    + eapply wt_path_deref_inv in H0.
+      destruct H0 as (ty1' & A1 & A2).
+      eapply wt_path_deref_inv in H.
+      destruct H as (ty1'' & A3 & A4).
+      exploit IHn. eauto. eapply A1. eapply A3. intros.
+      subst. rewrite A2 in A4. inv A4. auto.
+    + eapply wt_path_field_inv in H0 as (id & orgs & co & A1 & A2 & A3 & A4).
+      eapply wt_path_field_inv in H as (id1 & orgs1 & co1 & B1 & B2 & B3 & B4).
+      exploit IHn. eauto. eapply A1. eapply B1.
+      intros. inv H. rewrite A2 in B2. inv B2. rewrite A3 in B3. inv B3.
+      auto.
+    + eapply wt_path_downcast_inv in H0 as (id & orgs & co & A1 & A2 & A3 & A4 & A5).
+      eapply wt_path_downcast_inv in H as (id1 & orgs1 & co1 & B1 & B2 & B3 & B4 & B5).
+      rewrite A1 in B1. inv B1.
+      rewrite A3 in B3. inv B3. rewrite A4 in B4. inv B4. auto.
+Qed.
+
+      
+Lemma wt_path_app: forall phl2 phl1 ty1 ty2 ty3 ce,
+    wt_path ce ty1 phl1 ty2 ->
+    wt_path ce ty1 (phl1 ++ phl2) ty3 ->
+    wt_path ce ty2 phl2 ty3.
+Proof.
+  intro phl2. cut (exists n, length phl2 = n); eauto. intros (n & LEN).
+  generalize dependent phl2.
+  induction n; intros.
+  - eapply length_zero_iff_nil in LEN. subst.
+    rewrite app_nil_r in H0. exploit wt_path_det. eapply H. eapply H0.
+    intro. subst. econstructor.
+  - eapply length_S_inv in LEN.
+    destruct LEN as (l' & a & A & LEN). subst.
+    destruct a.
+    + rewrite app_assoc in H0.
+      eapply wt_path_deref_inv in H0.
+      destruct H0 as (ty1' & A1 & A2).
+      econstructor. eapply IHn; eauto. auto.
+    + rewrite app_assoc in H0.
+      eapply wt_path_field_inv in H0 as (id & orgs & co & A1 & A2 & A3 & A4).
+      econstructor; eauto.
+    + rewrite app_assoc in H0.
+      eapply wt_path_downcast_inv in H0 as (id & orgs & co & A1 & A2 & A3 & A4 & A5).
+      subst.
+      econstructor; eauto.
+Qed.
+
+Lemma wt_path_app_inv: forall phl2 phl1 ty1 ty3 ce,
+    wt_path ce ty1 (phl1 ++ phl2) ty3 ->
+    exists ty2,
+      wt_path ce ty1 phl1 ty2
+      /\ wt_path ce ty2 phl2 ty3.
+Proof.
+  intro phl2. cut (exists n, length phl2 = n); eauto. intros (n & LEN).
+  generalize dependent phl2.
+  induction n; intros.
+  - eapply length_zero_iff_nil in LEN. subst.
+    rewrite app_nil_r in H.
+    exists ty3. split; auto. econstructor.
+  - eapply length_S_inv in LEN.
+    destruct LEN as (l' & a & A & LEN). subst.
+    destruct a.
+    + rewrite app_assoc in H.
+      eapply wt_path_deref_inv in H.
+      destruct H as (ty1' & A1 & A2).
+      exploit IHn; eauto. intros (ty2' & B1 & B2).
+      exists ty2'. split; auto.
+      econstructor; eauto.
+    + rewrite app_assoc in H.
+      eapply wt_path_field_inv in H as (id & orgs & co & A1 & A2 & A3 & A4).
+      exploit IHn; eauto. intros (ty2' & B1 & B2).
+      exists ty2'. split; auto.
+      econstructor; eauto.
+    + rewrite app_assoc in H.
+      eapply wt_path_downcast_inv in H as (id & orgs & co & A1 & A2 & A3 & A4 & A5).
+      subst.
+      exploit IHn; eauto.
+      intros (ty2' & B1 & B2).
+      exists ty2'. split; auto.
+      econstructor; eauto.
+Qed.
+
+
+
+Lemma wt_place_wt_path: forall p e ce id l ty b,
+    wt_place (env_to_tenv e) ce p ->
+    path_of_place p = (id, l) ->
+    e ! id = Some (b, ty) ->
+    wt_path ce ty l (typeof_place p).
+Proof.
+  induction p; simpl; intros.
+  - inv H0. inv H.
+    unfold env_to_tenv in WT1.
+    rewrite PTree.gmap1 in WT1. rewrite H1 in WT1. inv WT1.
+    constructor.
+  - destruct (path_of_place p) eqn: POP. inv H0.
+    inv H. econstructor; eauto.
+    rewrite <- WT2. eauto.
+  - destruct (path_of_place p) eqn: POP. inv H0.
+    inv H. econstructor; eauto.
+  - destruct (path_of_place p) eqn: POP. inv H0.
+    inv H. rewrite WT2. econstructor; eauto.
+    rewrite <- WT2. eauto.
+Qed.    
+
+
+(** IMPORTANT TODO *)
+Lemma get_wt_footprint_wt: forall phl ty1 ty2 ce (WTPH: wt_path ce ty1 phl ty2) fp1 fp2,
+    wt_footprint ce ty1 fp1 ->
+    get_footprint phl fp1 = Some fp2 ->
+    wt_footprint ce ty2 fp2.
+Proof.
+  induction 1; intros; simpl in *.
+  - inv H0. auto.
+  - exploit get_footprint_app_inv; eauto.
+    intros (fp3 & A1 & A2). simpl in A2. destruct fp3; try congruence.
+    inv A2. exploit IHWTPH; eauto.
+    intros A2. inv A2. simpl in WP2. inv WP2. auto.
+  - exploit get_footprint_app_inv; eauto.
+    intros (fp3 & A1 & A2). simpl in A2. destruct fp3; try congruence.
+    destruct (find_fields fid fpl) eqn: FIND; try congruence.
+    repeat destruct p. inv A2.
+    exploit IHWTPH; eauto. intros A3. inv A3.
+    exploit find_fields_some; eauto.
+    intros (B1 & B2). subst.
+    exploit WT2; eauto.
+    intros (fty & C1 & C2 & C3).
+    rewrite WP2 in CO. inv CO.
+    rewrite WP3 in C1. inv C1.
+    auto.
+  - exploit get_footprint_app_inv; eauto.
+    intros (fp3 & A1 & A2). simpl in A2. destruct fp3; try congruence.
+    destruct ident_eq in A2; try congruence.
+    destruct list_eq_dec in A2; try congruence.
+    destruct ident_eq in A2; try congruence.
+    inv A2.
+    exploit IHWTPH; eauto. intros A3. inv A3.
+    rewrite WP2 in CO. inv CO.
+    rewrite WP3 in FTY. inv FTY. auto.
+Qed.    
+    
+(* A well typed footprint can imply all the sub-footprint's
+well-typedness and the path to htis footprint also is well-typed *) 
+Lemma get_wt_footprint_exists_wt: forall phl fp fp1 ty ce,
+    wt_footprint ce ty fp ->
+    get_footprint phl fp = Some fp1 ->
+    exists ty1, wt_footprint ce ty1 fp1
+           /\ wt_path ce ty phl ty1.
+Proof.
+  intros phl. cut (exists n, length phl = n); eauto. intros (n & LEN).
+  generalize dependent phl.
+  induction n; intros.
+  - eapply length_zero_iff_nil in LEN. subst.
+    simpl in *. inv H0.
+    exists ty. split; eauto.
+    econstructor.
+  - exploit length_S_inv; eauto.
+    intros (phl' & a & TYS & LEN1). subst.
+    exploit get_footprint_app_inv. eauto.
+    intros (fp3 & G1 & G2).
+    simpl in G2.
+    destruct a.
+    + destruct fp3; try congruence.
+      inv G2. exploit IHn; eauto.
+      intros (ty1 & A1 & A2).
+      inv A1.
+      exists ty0. split; auto. econstructor; eauto.      
+    + destruct fp3; try congruence.
+      destruct (find_fields fid fpl) eqn: A; try congruence.
+      repeat destruct p.
+      inv G2.
+      exploit find_fields_some; eauto. intros (A1 & A2). subst.
+      exploit IHn; eauto. intros (ty1 & W1 & W2).
+      inv W1.      
+      exploit WT2; eauto.
+      intros (fty & B1 & B2 & B3).
+      exists fty. split; auto.
+      econstructor; eauto. 
+    + destruct fp3; try congruence.
+      destruct ty0; try congruence.
+      destruct ident_eq; try congruence.
+      destruct list_eq_dec; try congruence.
+      destruct ident_eq; try congruence. subst.
+      inv G2. exploit IHn; eauto.
+      intros (ty1 & A1 & A2).
+      inv A1. exists fty. split; auto.
+      econstructor; eauto.
+Qed.
+      
+Lemma get_loc_footprint_map_different_local: forall id1 id2 phl1 phl2 fpm e b1 b2 ofs1 ofs2 fp1 fp2,
+    list_norepet (footprint_of_env e ++ flat_fp_map fpm) ->
+    id1 <> id2 ->
+    get_loc_footprint_map e (id1, phl1) fpm = Some (b1, ofs1, fp1) ->
+    get_loc_footprint_map e (id2, phl2) fpm = Some (b2, ofs2, fp2) ->
+    b1 <> b2 /\ ~ In b1 (footprint_flat fp2) /\ ~ In b2 (footprint_flat fp1).
+Proof.
+  intros until fp2. intros NOREP NEQ GFP1 GFP2.
+  simpl in *.
+  destruct (e!id1) eqn: A1; try congruence. destruct p.
+  destruct (e!id2) eqn: A2; try congruence. destruct p.
+  destruct (fpm!id1) eqn: B1; try congruence. 
+  destruct (fpm!id2) eqn: B2; try congruence.
+  exploit get_loc_footprint_in. eapply GFP1. intros IN1.
+  exploit get_loc_footprint_in. eapply GFP2. intros IN2.
+  eapply list_norepet_app in NOREP as (N1 & N2 & N3).
+  inv IN1; inv IN2.  
+  - repeat apply conj.
+    + eapply footprint_norepet_env_disjoint; eauto.
+    + intro. eapply N3.
+      eapply in_footprint_of_env. eapply A1.
+      eapply in_footprint_flat_fp_map. eapply B2.
+      eapply get_loc_footprint_incl. eapply GFP2. eapply H. auto.
+    + intro. eapply N3.
+      eapply in_footprint_of_env. eapply A2.
+      eapply in_footprint_flat_fp_map. eapply B1.
+      eapply get_loc_footprint_incl. eauto. eauto. auto.
+  - repeat apply conj.
+    + eapply N3.
+      eapply in_footprint_of_env. eauto.
+      eapply in_footprint_flat_fp_map. eapply B2. auto.
+    + intro. eapply N3.
+      eapply in_footprint_of_env. eapply A1.
+      eapply in_footprint_flat_fp_map. eapply B2.
+      eapply get_loc_footprint_incl. eauto. eauto. auto.
+    + intro.
+      eapply norepet_flat_fp_map_element_disjoint.
+      eapply B1. eapply B2. eauto. auto.
+      eapply get_loc_footprint_incl; eauto. eauto. auto.
+  - repeat apply conj.
+    + intro. subst. eapply N3.
+      eapply in_footprint_of_env. eapply A2.
+      eapply in_footprint_flat_fp_map. eapply B1. eauto. auto.
+    + intro. eapply norepet_flat_fp_map_element_disjoint.      
+      eapply B1. eapply B2. eauto. auto. eauto.
+      eapply get_loc_footprint_incl; eauto. eauto. 
+    + intro.
+      eapply N3.
+      eapply in_footprint_of_env. eapply A2.
+      eapply in_footprint_flat_fp_map. eapply B1.
+      eapply get_loc_footprint_incl. eauto. eauto. auto.
+  - repeat apply conj.
+    + intro. subst.
+      eapply norepet_flat_fp_map_element_disjoint.      
+      eapply B1. eapply B2. eauto. auto. eauto. eauto. auto.
+    + intro.
+      eapply norepet_flat_fp_map_element_disjoint.      
+      eapply B1. eapply B2. eauto. auto. eauto.
+      eapply get_loc_footprint_incl. eauto. eauto. auto.
+    + intro.
+      eapply norepet_flat_fp_map_element_disjoint.      
+      eapply B1. eapply B2. eauto. auto.
+      eapply get_loc_footprint_incl. eauto. eauto. eauto. auto.
+Qed.
+
+(** Properties of getting the footprint in disjoint paths *)
+
+Section COMP_ENV.
+
+Variable ce : composite_env.
+
+Hypothesis CONSISTENT: composite_env_consistent ce.
+
+Hypothesis COMP_RANGE: forall id co, ce ! id = Some co -> co_sizeof co <= Ptrofs.max_unsigned.
+Hypothesis COMP_LEN: forall id co, ce ! id = Some co -> list_length_z (co_members co) <= Int.max_unsigned.
+Hypothesis COMP_NOREP: forall id co, ce ! id = Some co -> list_norepet (name_members (co_members co)).
+
+
+(* The field type must be in the range of the struct it resides
+in. This lemma require consistent composite because the size of the
+struct is computed by co_sizeof instead of sizeof_struct *)
+Lemma field_offset_in_range_complete: forall ce co id ofs ty,
+    co_sv co = Struct ->
+    composite_consistent ce co ->
+    field_offset ce id (co_members co) = OK ofs ->
+    field_type id (co_members co) = OK ty ->
+    0 <= ofs /\ ofs + sizeof ce ty <= co_sizeof co.
+Proof.
+  intros.
+  exploit field_offset_in_range; eauto.
+  intros (S1 & S2). 
+  split. lia.
+  (* to show that sizeof_struct ce co0 <= co_sizeof co0 *)
+  erewrite co_consistent_sizeof; eauto.
+  erewrite co_consistent_alignof; eauto.
+  rewrite H. simpl.
+  generalize (sizeof_composite_pos ce0 Struct (co_members co)). simpl.
+  generalize (alignof_composite_pos ce0 (co_members co) Struct).
+  intros M1 M2. simpl in M1.
+  generalize (align_le (sizeof_struct ce0 (co_members co)) _ M1).
+  intros M3. lia.
+Qed.
+
+Lemma variant_field_offset_in_range_complete: forall ce co id ofs ty,
+    co_sv co = TaggedUnion ->
+    composite_consistent ce co ->
+    variant_field_offset ce id (co_members co) = OK ofs ->
+    field_type id (co_members co) = OK ty ->
+    4 <= ofs /\ ofs + sizeof ce ty <= co_sizeof co.
+Proof.
+  intros.
+  exploit variant_field_offset_in_range; eauto.
+  intros (S1 & S2). 
+  split. lia.
+  (* to show that sizeof_struct ce co0 <= co_sizeof co0 *)
+  erewrite co_consistent_sizeof; eauto.
+  erewrite co_consistent_alignof; eauto.
+  rewrite H. simpl.
+  generalize (sizeof_composite_pos ce0 TaggedUnion (co_members co)). simpl.
+  generalize (alignof_composite_pos ce0 (co_members co) TaggedUnion).
+  intros M1 M2. simpl in M1.
+  generalize (align_le (sizeof_variant ce0 (co_members co)) _ M1).
+  intros M3. lia.
+Qed.
+
+
+(* Two memory location (b1, ofs1) and (b2, ofs2) which have type ty1
+and ty2 are non-overlap *)
+Definition loc_disjoint (b1 b2: block) (ty1 ty2: type) (ofs1 ofs2: Z) : Prop :=
+  b1 <> b2 \/ ofs2 + sizeof ce ty2 <= ofs1 \/ ofs1 + sizeof ce ty1 <= ofs2.
+
+
+(** The memory location obtained from get_loc_footprint is either in
+    the range of [(b, ofs), (b, ofs+ sizeof ty)] or in the footprint
+    fp. Maybe this lemma require norepet of fp? Because
+    get_loc_footprint_disjoint_loc need this. *)
+Lemma get_loc_footprint_in_range: forall phl fp b ofs b1 ofs1 fp1 ty ty1,
+    wt_footprint ce ty fp ->
+    wt_path ce ty phl ty1 ->
+    ~ In b (footprint_flat fp) ->
+    (* no cycle in the footprint *)
+    list_norepet (footprint_flat fp) ->
+    get_loc_footprint phl fp b ofs = Some (b1, ofs1, fp1) ->
+    (b = b1 /\ ofs <= ofs1 /\ ofs1 + sizeof ce ty1 <= ofs + sizeof ce ty)
+    \/ (b <> b1 /\ In b1 (footprint_flat fp)).
+Proof.
+  intro phl. cut (exists n, length phl = n); eauto. intros (n & LEN).
+  generalize dependent phl.
+  induction n; intros until ty1; intros WTFP WTPH NIN NOREP GFP; simpl in *.  
+  - eapply length_zero_iff_nil in LEN. subst. simpl in *.
+    inv GFP. eapply wt_path_nil_inv in WTPH. subst. left.
+    split; auto. lia.    
+  - eapply length_S_inv in LEN. destruct LEN as (phl' & ph & APP & LEN).
+    subst. 
+    exploit get_loc_footprint_app_inv. eauto.
+    intros (b2 & ofs2 & fp3 & A1 & A2).
+    simpl in A2.
+    destruct ph.
+    + destruct fp3; try congruence.
+      eapply wt_path_deref_inv in WTPH as (ty' & WTPH & TYDEF).
+      eapply type_deref_some in TYDEF. subst.
+      inv A2.
+      exploit get_loc_footprint_norepet; eauto.
+      simpl. intros (C1 & C2). eapply Decidable.not_or in C2. destruct C2 as (C2 & C3).
+      exploit IHn. eauto. eapply WTFP. eauto. eauto. eauto. eauto.
+      intros [B1 | B2].
+      * destruct B1. subst.
+        right. split; auto.
+        eapply get_loc_footprint_incl; eauto. simpl. auto.
+      * destruct B2. right. split.
+        intro. subst. eapply NIN. eapply get_loc_footprint_incl. eapply A1. 
+        simpl. auto.
+        eapply get_loc_footprint_incl. eapply A1. simpl. auto.
+    + destruct fp3; try congruence.
+      destruct (find_fields fid fpl) eqn: FIND; try congruence.
+      repeat destruct p.
+      inv A2. eapply wt_path_field_inv in WTPH as (id1 & orgs & co & WTPH & CO & FTY & STRUCT).
+      exploit find_fields_some; eauto. intros (C1 & C2). subst.
+      exploit get_loc_footprint_norepet. eauto. eapply A1. auto.
+      intros (N1 & N2).
+      exploit get_wt_footprint_wt. eauto. eapply WTFP. eapply get_loc_footprint_eq. eauto.
+      intros WTFP1. inv WTFP1.
+      exploit WT2; eauto. intros (fty & FTY1 & FOFS & WTFP2). 
+      rewrite CO in CO0. inv CO0.
+      rewrite FTY in FTY1. inv FTY1.
+      exploit IHn. eauto. eapply WTFP. all: eauto.
+      intros [B1 | B2].
+      * destruct B1. subst.
+        left. split; auto.
+        simpl in H0. rewrite CO in H0.
+        exploit field_offset_in_range_complete; eauto. lia.
+      * destruct B2. right. split; auto.
+    + destr_fp_enum fp3 ty0.
+      inv A2.
+      eapply wt_path_downcast_inv in WTPH as (id1 & orgs1 & co & TY & WTPH & CO & FTY & ENUM).
+      inv TY.
+      exploit get_loc_footprint_norepet. eauto. eapply A1. auto.
+      intros (N1 & N2).      
+      exploit get_wt_footprint_wt. eauto. eapply WTFP. eapply get_loc_footprint_eq. eauto.
+      intros WTFP1. inv WTFP1.
+      rewrite CO in CO0. inv CO0. rewrite FTY in FTY0. inv FTY0.
+      exploit IHn. eauto. eapply WTFP. all: eauto.
+      intros [B1 | B2].
+      * destruct B1. subst.
+        left. split; auto.
+        simpl in H0. rewrite CO in H0.
+        exploit variant_field_offset_in_range_complete; eauto. lia.
+      * destruct B2. right. split; auto.
+Qed.
+
+(** IMPORTANT TODO: This lemma says that the (memory locations,
+   footprint) obtained from different location are different, no
+   matter what paths it resides in. *)
+Lemma get_loc_footprint_disjoint_loc: forall phl1 phl2 b1 b2 ty1 ty2 ofs1 ofs2 b1' b2' ofs1' ofs2' ty1' ty2' fp1 fp2 fp1' fp2',
+    loc_disjoint b1 b2 ty1 ty2 ofs1 ofs2 ->
+    (* What relation between ty1 and ty1'?? We can prove sizeof
+          ty1 = sizeof ty1'*)
+    wt_footprint ce ty1 fp1 ->
+    wt_footprint ce ty2 fp2 ->
+    wt_path ce ty1 phl1 ty1' ->
+    wt_path ce ty2 phl2 ty2' ->
+    get_loc_footprint phl1 fp1 b1 ofs1 = Some (b1', ofs1', fp1') ->
+    get_loc_footprint phl2 fp2 b2 ofs2 = Some (b2', ofs2', fp2') ->
+    list_disjoint (footprint_flat fp1) (footprint_flat fp2) ->
+    list_norepet (footprint_flat fp1) ->
+    list_norepet (footprint_flat fp2) ->
+    ~ In b1 (footprint_flat fp1) ->
+    ~ In b2 (footprint_flat fp2) ->
+    ~ In b1 (footprint_flat fp2) ->
+    ~ In b2 (footprint_flat fp1) ->
+    loc_disjoint b1' b2' ty1' ty2' ofs1' ofs2'
+    /\ ~ In b1' (footprint_flat fp2')
+    /\ ~ In b2' (footprint_flat fp1')
+    /\ list_disjoint (footprint_flat fp1') (footprint_flat fp2').
+Proof.
+  induction phl1; intros until fp2'; intros DIS1 WT1 WT2 WTPH1 WTPH2 G1 G2 DIS2 NOREP1 NOREP2 IN1 IN2 IN3 IN4.
+  - simpl in G1. inv G1.
+    exploit get_loc_footprint_in_range. eapply WT2. eapply WTPH2. 
+    3: eapply G2. eauto. eauto.
+    intros [[A1 [A2 A3]]|[A1 A2]].
+    + subst. repeat apply conj.
+      * destruct DIS1; red; auto.
+        right. 
+        generalize sizeof_pos. intros.
+        destruct H. lia.
+        eapply wt_path_nil_inv in WTPH1. subst. lia.
+      * intro. apply IN3.
+        eapply get_loc_footprint_incl; eauto.
+      * auto.  
+      * red. intros. intro.
+        eapply DIS2. eauto. eapply get_loc_footprint_incl; eauto.
+        auto.
+    + repeat apply conj.
+      * red. left.
+        intro. subst. congruence.
+      * intro. apply IN3.
+        eapply get_loc_footprint_incl; eauto.
+      * intro. eapply DIS2; eauto.
+      * red. intros. intro.
+        eapply DIS2. eauto. eapply get_loc_footprint_incl; eauto.
+        auto.
+  - replace (a::phl1) with ((a::nil) ++ phl1) in G1 by auto.
+    exploit get_loc_footprint_app_inv. eauto.
+    intros (b3 & ofs3 & fp3 & B1 & B2).
+    (* show fp3 is well-typed *)
+    exploit get_wt_footprint_exists_wt. eapply WT1.
+    eapply get_loc_footprint_eq; eauto.
+    intros (ty3 & C1 & C2).
+    (* show (b3, ofs3) has no overlap with (b2,ofs2) *)
+    assert (DIS3: loc_disjoint b3 b2 ty3 ty2 ofs3 ofs2).
+    { exploit get_loc_footprint_in_range. eapply WT1. eapply C2.
+      3: eapply B1. eauto.
+      eauto. intros [[A1 [A2 A3]]|[A1 A2]].
+      - subst. 
+        destruct DIS1; red; auto.
+        right. 
+        generalize sizeof_pos. intros.
+        destruct H. lia. lia.
+      - red. left.
+        intro. subst. congruence. }
+    exploit get_loc_footprint_norepet. 2: eapply B1. eauto. eauto.
+    intros (D1 & D2).
+    eapply IHphl1.
+    eapply DIS3. 1-6: eauto.
+    eapply wt_path_app. eauto. simpl. auto.
+    (* disjointness between fp3 and fp2 *)
+    red. intros. intro. eapply DIS2.
+    eapply get_loc_footprint_incl; eauto. eauto. auto.
+    eauto. eauto.
+    (* four notin *)
+    eauto. eauto.
+    (* prove b3 is not in fp2 *)
+    exploit get_loc_footprint_in_range. eapply WT1. eapply C2. 
+    eapply IN1. eauto. eauto.
+    intros [[A1 [A2 A3]]|[A1 A2]].
+    subst. eauto.
+    intro. eapply DIS2. eauto. eauto. auto.
+    (* b2 is not in fp3 *)
+    intro. eapply IN4. eapply get_loc_footprint_incl. eauto.
+    auto.
+Qed.
+
+
+
+(* Some properties of wt_footprint. This lemma says that the
+(location, footprint) pairs obtained form disjoint paths are disjoint,
+i.e., the locations are disjoint and the footprints have no equal
+blocks. To express the disjointness of locaitons, we also need the
+type of the footprint to get its size, so we add wt_footprint premises
+in this lemma. This lemma is hard to refactor because we do induction
+on phl instead of its length. *)
+Lemma get_loc_footprint_disjoint_paths: forall phl1 phl2 fp b ofs b1 b2 ofs1 ofs2 fp1 fp2 ty ty1 ty2,
+    paths_disjoint phl1 phl2 ->
+    list_norepet (footprint_flat fp) ->
+    wt_footprint ce ty fp ->
+    wt_path ce ty phl1 ty1 ->
+    wt_path ce ty phl2 ty2 ->
+    get_loc_footprint phl1 fp b ofs = Some (b1, ofs1, fp1) ->
+    get_loc_footprint phl2 fp b ofs = Some (b2, ofs2, fp2) ->
+    (~ In b (footprint_flat fp)) ->
+    (* footprint locations are disjoint *)
+    loc_disjoint b1 b2 ty1 ty2 ofs1 ofs2
+    (* location and footprint are disjoint *)
+    /\ (~ In b1 (footprint_flat fp2))
+    /\ (~ In b2 (footprint_flat fp1))
+    (* b1 may be equal to b2 so we cannot say b1::fp1 is disjoint with b2::fp2 *)
+    /\ list_disjoint (footprint_flat fp1) (footprint_flat fp2).
+Proof.
+  induction phl1; intros until ty2.
+  - intros. inv H.
+  - intros DIS NOREP WT WTPH1 WTPH2 G1 G2 IN.
+    inv DIS.
+    + replace (a::phl1) with ((a::nil) ++ phl1) in WTPH1; auto.
+      replace (p2::l2) with ((p2::nil) ++ l2) in WTPH2; auto.
+      exploit wt_path_app_inv. eapply WTPH1.
+      intros (ty1' & WTPH1' & WTPH1'').
+      exploit wt_path_app_inv. eapply WTPH2.
+      intros (ty2' & WTPH2' & WTPH2'').
+      simpl in G1, G2.
+      destruct a; destruct p2; destruct fp; simpl in *; try congruence.
+      (* Case1: disjoint struct fields *)
+      * destruct (find_fields fid fpl) eqn: FIND1; try congruence. repeat destruct p.
+        destruct (find_fields fid0 fpl) eqn: FIND2; try congruence. repeat destruct p.
+        exploit find_fields_some; eauto. intros (A1 & A2). subst.
+        exploit find_fields_some. eapply FIND1. intros (A3 & A4). subst.
+        (* get the subfield types and offsets *)
+        inv WT.
+        exploit WT2. eapply FIND1. intros (fty1 & FTY1 & FOFS1 & WST1).
+        exploit WT2. eapply FIND2. intros (fty2 & FTY2 & FOFS2 & WST2).
+        (* tediously get ty1' and ty2' *)
+        erewrite <- (app_nil_l [ph_field i]) in WTPH1'.
+        eapply wt_path_field_inv in WTPH1' as (id1' & orgs1' & co1' & WTPH1' & CO1' & FTY1' & STR1').
+        eapply wt_path_nil_inv in WTPH1'. inv WTPH1'. rewrite CO1' in CO. inv CO.
+        rewrite FTY1' in FTY1. inv FTY1.
+        erewrite <- (app_nil_l [ph_field i0]) in WTPH2'.
+        eapply wt_path_field_inv in WTPH2' as (id2' & orgs2' & co2' & WTPH2' & CO2' & FTY2' & STR2').
+        eapply wt_path_nil_inv in WTPH2'. inv WTPH2'. rewrite CO2' in CO1'. inv CO1'.
+        rewrite FTY2' in FTY2. inv FTY2.
+        (* end of getting ty1' and ty2' *)
+        (* field offset no overlap to get loc_disjoint *)
+        exploit field_offset_no_overlap_simplified.
+        eapply FOFS1. eauto. eapply FOFS2. eauto.
+        congruence.
+        intros FOFS_DIS.
+        assert (LOC_DIS: loc_disjoint b b fty1 fty2 (ofs + z) (ofs + z0)).
+        { red. right. lia. }
+        (* use get_loc_footprint_disjoint_loc *)        
+        exploit get_loc_footprint_disjoint_loc. eapply LOC_DIS. eauto. eauto.
+        all: eauto.
+        (* prove f and f0 are disjoint using fpl norepet *)
+        eapply footprint_norepet_fields_disjoint; eauto.
+        congruence.
+        (* norepet *)
+        (* easy because f and f0 are in fpl and fpl is norepet *)
+        eapply footprint_norepet_fields_norepet; eauto.
+        eapply footprint_norepet_fields_norepet; eauto.
+        intro. eapply IN. eapply in_flat_map. eauto.
+        intro. eapply IN. eapply in_flat_map. eauto.
+        intro. eapply IN. eapply in_flat_map. eauto.
+        intro. eapply IN. eapply in_flat_map. eauto.
+      * destruct ty0; try congruence.
+        destruct ty3; try congruence.
+        repeat destruct ident_eq in *; try congruence;
+        repeat destruct list_eq_dec; try congruence. 
+    + replace (a::phl1) with ((a::nil)++phl1) in * by auto.
+      replace (a::l2) with ((a::nil)++l2) in * by auto.
+      exploit wt_path_app_inv. eapply WTPH1.
+      intros (ty1' & WTPH1' & WTPH1'').
+      exploit wt_path_app_inv. eapply WTPH2.
+      intros (ty2' & WTPH2' & WTPH2'').
+      exploit get_loc_footprint_app_inv. eapply G1.
+      intros (b3 & ofs3 & fp3 & C1 & C2).
+      exploit get_loc_footprint_app_inv. eapply G2.
+      intros (b4 & ofs4 & fp4 & C3 & C4).
+      rewrite C1 in C3. inv C3.
+      assert (WTFP4: wt_footprint ce ty1' fp4).
+      { exploit get_wt_footprint_wt. eapply WTPH1'. eapply WT.
+        eapply get_loc_footprint_eq; eauto.
+        eauto. }
+      exploit wt_path_det. eapply WTPH1'. eauto. intros. subst.
+      (* use I.H. *)
+      exploit get_loc_footprint_norepet. eapply NOREP. eauto. eauto.
+      intros (D1 & D2).            
+      exploit IHphl1; eauto.      
+Qed.
+
+End COMP_ENV.
+
+  
